QCP_examples/humaneval/spec_logic_rewrite_c_files/C_78_goal.v
@@ -1,0 +1,731 @@
+Require Import Coq.ZArith.ZArith.
+Require Import Coq.Bool.Bool.
+Require Import Coq.Strings.String.
+Require Import Coq.Strings.Ascii.
+Require Import Coq.Lists.List.
+Require Import Coq.Classes.RelationClasses.
+Require Import Coq.Classes.Morphisms.
+Require Import Coq.micromega.Psatz.
+Require Import Coq.Sorting.Permutation.
+From AUXLib Require Import int_auto Axioms Feq Idents ListLib VMap.
+Require Import SetsClass.SetsClass. Import SetsNotation.
+From SimpleC.SL Require Import Mem SeparationLogic.
+Require Import Logic.LogicGenerator.demo932.Interface.
+Local Open Scope Z_scope.
+Local Open Scope sets.
+Local Open Scope string_scope.
+Local Open Scope list.
+Import naive_C_Rules.
+Require Import SimpleC.StdLib.string_lib.
+Require Import coins_78.
+Local Open Scope sac.
+From SimpleC.EE.QCP_demos_LLM Require Import char_array_strategy_goal.
+From SimpleC.EE.QCP_demos_LLM Require Import char_array_strategy_proof.
+From SimpleC.StdLib Require Import string_strategy_goal.
+From SimpleC.StdLib Require Import string_strategy_proof.
+
+(*----- Function hex_key -----*)
+
+Definition hex_key_safety_wit_1 := 
+forall (num_pre: Z) (str_l: (@list Z)) (PreH1 : (valid_string str_l )) (PreH2 : (all_ascii str_l )) (PreH3 : (problem_78_pre_z str_l )) (PreH4 : (hex_count_safe_78 str_l )) (PreH5 : (key_payload_safe_78 )) (PreH6 : ((string_length (str_l)) < INT_MAX)) ,
+  (store_stringLit (LitMap (("2357BD"%string))) ("2357BD"%string) )
+  **  (GlobalStrings_missing LitMap (cons (("2357BD"%string)) ((@nil string))) )
+  **  ((( &( "key" ) )) # Ptr  |->_)
+  **  ((( &( "num" ) )) # Ptr  |-> num_pre)
+  **  (store_string num_pre str_l )
+|--
+  “ (0 <= INT_MAX) ” 
+  &&  “ ((INT_MIN) <= 0) ”
+.
+
+Definition hex_key_safety_wit_2 := 
+forall (num_pre: Z) (str_l: (@list Z)) (key: Z) (retval: Z) (PreH1 : (retval = (string_length (str_l)))) (PreH2 : (0 <= ((string_length (key_payload_78)) + 1 ))) (PreH3 : (0 <= ((string_length (str_l)) + 1 ))) (PreH4 : (key = (key_ptr_78 (LitMap)))) (PreH5 : (valid_string str_l )) (PreH6 : (all_ascii str_l )) (PreH7 : (problem_78_pre_z str_l )) (PreH8 : (hex_count_safe_78 str_l )) (PreH9 : (key_payload_safe_78 )) (PreH10 : ((string_length (str_l)) < INT_MAX)) ,
+  ((( &( "out" ) )) # Int  |->_)
+  **  (store_string num_pre str_l )
+  **  (CharArray.full key ((string_length (key_payload_78)) + 1 ) (c_string (key_payload_78)) )
+  **  ((( &( "n" ) )) # Int  |-> retval)
+  **  ((( &( "num" ) )) # Ptr  |-> num_pre)
+  **  ((( &( "key" ) )) # Ptr  |-> key)
+  **  (GlobalStrings_missing LitMap all_key_literals_78 )
+|--
+  “ (0 <= INT_MAX) ” 
+  &&  “ ((INT_MIN) <= 0) ”
+.
+
+Definition hex_key_safety_wit_3 := 
+forall (num_pre: Z) (str_l: (@list Z)) (key: Z) (retval: Z) (PreH1 : (retval = (string_length (str_l)))) (PreH2 : (0 <= ((string_length (key_payload_78)) + 1 ))) (PreH3 : (0 <= ((string_length (str_l)) + 1 ))) (PreH4 : (key = (key_ptr_78 (LitMap)))) (PreH5 : (valid_string str_l )) (PreH6 : (all_ascii str_l )) (PreH7 : (problem_78_pre_z str_l )) (PreH8 : (hex_count_safe_78 str_l )) (PreH9 : (key_payload_safe_78 )) (PreH10 : ((string_length (str_l)) < INT_MAX)) ,
+  ((( &( "i" ) )) # Int  |->_)
+  **  ((( &( "out" ) )) # Int  |-> 0)
+  **  (store_string num_pre str_l )
+  **  (CharArray.full key ((string_length (key_payload_78)) + 1 ) (c_string (key_payload_78)) )
+  **  ((( &( "n" ) )) # Int  |-> retval)
+  **  ((( &( "num" ) )) # Ptr  |-> num_pre)
+  **  ((( &( "key" ) )) # Ptr  |-> key)
+  **  (GlobalStrings_missing LitMap all_key_literals_78 )
+|--
+  “ (0 <= INT_MAX) ” 
+  &&  “ ((INT_MIN) <= 0) ”
+.
+
+Definition hex_key_safety_wit_4 := 
+forall (num_pre: Z) (str_l: (@list Z)) (out: Z) (i: Z) (n: Z) (key: Z) (retval: Z) (PreH1 : (strchr_result key_payload_78 (Znth i (c_string (str_l)) 0) retval key )) (PreH2 : (0 <= ((string_length (key_payload_78)) + 1 ))) (PreH3 : (0 <= ((string_length (str_l)) + 1 ))) (PreH4 : (i < n)) (PreH5 : (key = (key_ptr_78 (LitMap)))) (PreH6 : (n = (string_length (str_l)))) (PreH7 : (0 <= i)) (PreH8 : (i <= n)) (PreH9 : (0 <= out)) (PreH10 : (out <= i)) (PreH11 : (valid_string str_l )) (PreH12 : (all_ascii str_l )) (PreH13 : (problem_78_pre_z str_l )) (PreH14 : (hex_count_safe_78 str_l )) (PreH15 : (key_payload_safe_78 )) (PreH16 : ((string_length (str_l)) < INT_MAX)) (PreH17 : (hex_count_state_78 str_l i out )) ,
+  (store_string key key_payload_78 )
+  **  (CharArray.full num_pre ((string_length (str_l)) + 1 ) (c_string (str_l)) )
+  **  ((( &( "found" ) )) # Ptr  |-> retval)
+  **  ((( &( "ch" ) )) # Int  |-> (Znth i (c_string (str_l)) 0))
+  **  ((( &( "num" ) )) # Ptr  |-> num_pre)
+  **  ((( &( "key" ) )) # Ptr  |-> key)
+  **  ((( &( "n" ) )) # Int  |-> n)
+  **  ((( &( "i" ) )) # Int  |-> i)
+  **  ((( &( "out" ) )) # Int  |-> out)
+  **  (GlobalStrings_missing LitMap all_key_literals_78 )
+|--
+  “ (0 <= INT_MAX) ” 
+  &&  “ ((INT_MIN) <= 0) ”
+.
+
+Definition hex_key_safety_wit_5 := 
+forall (num_pre: Z) (str_l: (@list Z)) (out: Z) (i: Z) (n: Z) (key: Z) (retval: Z) (PreH1 : (retval <> 0)) (PreH2 : (strchr_result key_payload_78 (Znth i (c_string (str_l)) 0) retval key )) (PreH3 : (0 <= ((string_length (key_payload_78)) + 1 ))) (PreH4 : (0 <= ((string_length (str_l)) + 1 ))) (PreH5 : (i < n)) (PreH6 : (key = (key_ptr_78 (LitMap)))) (PreH7 : (n = (string_length (str_l)))) (PreH8 : (0 <= i)) (PreH9 : (i <= n)) (PreH10 : (0 <= out)) (PreH11 : (out <= i)) (PreH12 : (valid_string str_l )) (PreH13 : (all_ascii str_l )) (PreH14 : (problem_78_pre_z str_l )) (PreH15 : (hex_count_safe_78 str_l )) (PreH16 : (key_payload_safe_78 )) (PreH17 : ((string_length (str_l)) < INT_MAX)) (PreH18 : (hex_count_state_78 str_l i out )) ,
+  (store_string key key_payload_78 )
+  **  (CharArray.full num_pre ((string_length (str_l)) + 1 ) (c_string (str_l)) )
+  **  ((( &( "found" ) )) # Ptr  |-> retval)
+  **  ((( &( "ch" ) )) # Int  |-> (Znth i (c_string (str_l)) 0))
+  **  ((( &( "num" ) )) # Ptr  |-> num_pre)
+  **  ((( &( "key" ) )) # Ptr  |-> key)
+  **  ((( &( "n" ) )) # Int  |-> n)
+  **  ((( &( "i" ) )) # Int  |-> i)
+  **  ((( &( "out" ) )) # Int  |-> out)
+  **  (GlobalStrings_missing LitMap all_key_literals_78 )
+|--
+  “ ((out + 1 ) <= INT_MAX) ” 
+  &&  “ ((INT_MIN) <= (out + 1 )) ”
+.
+
+Definition hex_key_safety_wit_6 := 
+forall (num_pre: Z) (str_l: (@list Z)) (out: Z) (i: Z) (n: Z) (key: Z) (retval: Z) (PreH1 : (retval <> 0)) (PreH2 : (strchr_result key_payload_78 (Znth i (c_string (str_l)) 0) retval key )) (PreH3 : (0 <= ((string_length (key_payload_78)) + 1 ))) (PreH4 : (0 <= ((string_length (str_l)) + 1 ))) (PreH5 : (i < n)) (PreH6 : (key = (key_ptr_78 (LitMap)))) (PreH7 : (n = (string_length (str_l)))) (PreH8 : (0 <= i)) (PreH9 : (i <= n)) (PreH10 : (0 <= out)) (PreH11 : (out <= i)) (PreH12 : (valid_string str_l )) (PreH13 : (all_ascii str_l )) (PreH14 : (problem_78_pre_z str_l )) (PreH15 : (hex_count_safe_78 str_l )) (PreH16 : (key_payload_safe_78 )) (PreH17 : ((string_length (str_l)) < INT_MAX)) (PreH18 : (hex_count_state_78 str_l i out )) ,
+  (store_string key key_payload_78 )
+  **  (CharArray.full num_pre ((string_length (str_l)) + 1 ) (c_string (str_l)) )
+  **  ((( &( "found" ) )) # Ptr  |-> retval)
+  **  ((( &( "ch" ) )) # Int  |-> (Znth i (c_string (str_l)) 0))
+  **  ((( &( "num" ) )) # Ptr  |-> num_pre)
+  **  ((( &( "key" ) )) # Ptr  |-> key)
+  **  ((( &( "n" ) )) # Int  |-> n)
+  **  ((( &( "i" ) )) # Int  |-> i)
+  **  ((( &( "out" ) )) # Int  |-> out)
+  **  (GlobalStrings_missing LitMap all_key_literals_78 )
+|--
+  “ (1 <= INT_MAX) ” 
+  &&  “ ((INT_MIN) <= 1) ”
+.
+
+Definition hex_key_safety_wit_7 := 
+forall (num_pre: Z) (str_l: (@list Z)) (key: Z) (n: Z) (i: Z) (out: Z) (ch: Z) (PreH1 : (key = (key_ptr_78 (LitMap)))) (PreH2 : (n = (string_length (str_l)))) (PreH3 : (0 <= i)) (PreH4 : (i < n)) (PreH5 : (0 <= out)) (PreH6 : (out <= (i + 1 ))) (PreH7 : (0 <= ch)) (PreH8 : (ch <= 127)) (PreH9 : (valid_string str_l )) (PreH10 : (all_ascii str_l )) (PreH11 : (problem_78_pre_z str_l )) (PreH12 : (hex_count_safe_78 str_l )) (PreH13 : (key_payload_safe_78 )) (PreH14 : ((string_length (str_l)) < INT_MAX)) (PreH15 : (hex_hit_step_78 str_l i out )) (PreH16 : (hex_count_state_78 str_l (i + 1 ) out )) ,
+  ((( &( "num" ) )) # Ptr  |-> num_pre)
+  **  ((( &( "key" ) )) # Ptr  |-> key)
+  **  ((( &( "n" ) )) # Int  |-> n)
+  **  ((( &( "i" ) )) # Int  |-> i)
+  **  ((( &( "out" ) )) # Int  |-> out)
+  **  (store_string num_pre str_l )
+  **  (store_string key key_payload_78 )
+  **  (GlobalStrings_missing LitMap all_key_literals_78 )
+|--
+  “ ((i + 1 ) <= INT_MAX) ” 
+  &&  “ ((INT_MIN) <= (i + 1 )) ”
+.
+
+Definition hex_key_safety_wit_8 := 
+forall (num_pre: Z) (str_l: (@list Z)) (key: Z) (n: Z) (i: Z) (out: Z) (ch: Z) (PreH1 : (key = (key_ptr_78 (LitMap)))) (PreH2 : (n = (string_length (str_l)))) (PreH3 : (0 <= i)) (PreH4 : (i < n)) (PreH5 : (0 <= out)) (PreH6 : (out <= i)) (PreH7 : (0 <= ch)) (PreH8 : (ch <= 127)) (PreH9 : (valid_string str_l )) (PreH10 : (all_ascii str_l )) (PreH11 : (problem_78_pre_z str_l )) (PreH12 : (hex_count_safe_78 str_l )) (PreH13 : (key_payload_safe_78 )) (PreH14 : ((string_length (str_l)) < INT_MAX)) (PreH15 : (hex_miss_step_78 str_l i out )) (PreH16 : (hex_count_state_78 str_l (i + 1 ) out )) ,
+  ((( &( "num" ) )) # Ptr  |-> num_pre)
+  **  ((( &( "key" ) )) # Ptr  |-> key)
+  **  ((( &( "n" ) )) # Int  |-> n)
+  **  ((( &( "i" ) )) # Int  |-> i)
+  **  ((( &( "out" ) )) # Int  |-> out)
+  **  (store_string num_pre str_l )
+  **  (store_string key key_payload_78 )
+  **  (GlobalStrings_missing LitMap all_key_literals_78 )
+|--
+  “ ((i + 1 ) <= INT_MAX) ” 
+  &&  “ ((INT_MIN) <= (i + 1 )) ”
+.
+
+Definition hex_key_entail_wit_1 := 
+(
+forall (num_pre: Z) (str_l: (@list Z)) (PreH1 : (valid_string str_l )) (PreH2 : (all_ascii str_l )) (PreH3 : (problem_78_pre_z str_l )) (PreH4 : (hex_count_safe_78 str_l )) (PreH5 : (key_payload_safe_78 )) (PreH6 : ((string_length (str_l)) < INT_MAX)) ,
+  (store_stringLit (LitMap (("2357BD"%string))) ("2357BD"%string) )
+  **  (GlobalStrings_missing LitMap (cons (("2357BD"%string)) ((@nil string))) )
+  **  (store_string num_pre str_l )
+|--
+  “ (((LitMap (("2357BD"%string))) + (0 * sizeof(CHAR) ) ) = (key_ptr_78 (LitMap))) ” 
+  &&  “ (valid_string str_l ) ” 
+  &&  “ (all_ascii str_l ) ” 
+  &&  “ (problem_78_pre_z str_l ) ” 
+  &&  “ (hex_count_safe_78 str_l ) ” 
+  &&  “ (key_payload_safe_78 ) ” 
+  &&  “ ((string_length (str_l)) < INT_MAX) ”
+  &&  (store_string num_pre str_l )
+  **  (store_string ((LitMap (("2357BD"%string))) + (0 * sizeof(CHAR) ) ) key_payload_78 )
+  **  (GlobalStrings_missing LitMap all_key_literals_78 )
+) \/
+(
+forall (str_l: (@list Z)) (PreH1 : (0 <= ((string_length (str_l)) + 1 ))) (PreH2 : (valid_string str_l )) (PreH3 : (all_ascii str_l )) (PreH4 : (problem_78_pre_z str_l )) (PreH5 : (hex_count_safe_78 str_l )) (PreH6 : (key_payload_safe_78 )) (PreH7 : ((string_length (str_l)) < INT_MAX)) ,
+  (GlobalStrings LitMap )
+|--
+  “ (((LitMap (("2357BD"%string))) + (0 * sizeof(CHAR) ) ) = (key_ptr_78 (LitMap))) ”
+  &&  (CharArray.full ((LitMap (("2357BD"%string))) + (0 * sizeof(CHAR) ) ) ((string_length (key_payload_78)) + 1 ) (c_string (key_payload_78)) )
+  **  (GlobalStrings_missing LitMap all_key_literals_78 )
+).
+
+Definition hex_key_entail_wit_1_split_goal_1 := 
+forall (str_l: (@list Z)) (PreH1 : (0 <= ((string_length (str_l)) + 1 ))) (PreH2 : (valid_string str_l )) (PreH3 : (all_ascii str_l )) (PreH4 : (problem_78_pre_z str_l )) (PreH5 : (hex_count_safe_78 str_l )) (PreH6 : (key_payload_safe_78 )) (PreH7 : ((string_length (str_l)) < INT_MAX)) ,
+  (GlobalStrings LitMap )
+|--
+  “ (((LitMap (("2357BD"%string))) + (0 * sizeof(CHAR) ) ) = (key_ptr_78 (LitMap))) ”
+.
+
+Definition hex_key_entail_wit_1_split_goal_spatial := 
+forall (str_l: (@list Z)) (PreH1 : (0 <= ((string_length (str_l)) + 1 ))) (PreH2 : (valid_string str_l )) (PreH3 : (all_ascii str_l )) (PreH4 : (problem_78_pre_z str_l )) (PreH5 : (hex_count_safe_78 str_l )) (PreH6 : (key_payload_safe_78 )) (PreH7 : ((string_length (str_l)) < INT_MAX)) ,
+  (GlobalStrings LitMap )
+|--
+  (CharArray.full ((LitMap (("2357BD"%string))) + (0 * sizeof(CHAR) ) ) ((string_length (key_payload_78)) + 1 ) (c_string (key_payload_78)) )
+  **  (GlobalStrings_missing LitMap all_key_literals_78 )
+.
+
+Definition hex_key_entail_wit_2 := 
+(
+forall (num_pre: Z) (str_l: (@list Z)) (key: Z) (retval: Z) (PreH1 : (retval = (string_length (str_l)))) (PreH2 : (0 <= ((string_length (key_payload_78)) + 1 ))) (PreH3 : (0 <= ((string_length (str_l)) + 1 ))) (PreH4 : (key = (key_ptr_78 (LitMap)))) (PreH5 : (valid_string str_l )) (PreH6 : (all_ascii str_l )) (PreH7 : (problem_78_pre_z str_l )) (PreH8 : (hex_count_safe_78 str_l )) (PreH9 : (key_payload_safe_78 )) (PreH10 : ((string_length (str_l)) < INT_MAX)) ,
+  (store_string num_pre str_l )
+  **  (CharArray.full key ((string_length (key_payload_78)) + 1 ) (c_string (key_payload_78)) )
+  **  (GlobalStrings_missing LitMap all_key_literals_78 )
+|--
+  “ (key = (key_ptr_78 (LitMap))) ” 
+  &&  “ (retval = (string_length (str_l))) ” 
+  &&  “ (0 <= 0) ” 
+  &&  “ (0 <= retval) ” 
+  &&  “ (0 <= 0) ” 
+  &&  “ (0 <= 0) ” 
+  &&  “ (valid_string str_l ) ” 
+  &&  “ (all_ascii str_l ) ” 
+  &&  “ (problem_78_pre_z str_l ) ” 
+  &&  “ (hex_count_safe_78 str_l ) ” 
+  &&  “ (key_payload_safe_78 ) ” 
+  &&  “ ((string_length (str_l)) < INT_MAX) ” 
+  &&  “ (hex_count_state_78 str_l 0 0 ) ”
+  &&  (store_string num_pre str_l )
+  **  (store_string key key_payload_78 )
+  **  (GlobalStrings_missing LitMap all_key_literals_78 )
+) \/
+(
+forall (str_l: (@list Z)) (key: Z) (retval: Z) (PreH1 : (retval = (string_length (str_l)))) (PreH2 : (0 <= ((string_length (key_payload_78)) + 1 ))) (PreH3 : (0 <= ((string_length (str_l)) + 1 ))) (PreH4 : (key = (key_ptr_78 (LitMap)))) (PreH5 : (valid_string str_l )) (PreH6 : (all_ascii str_l )) (PreH7 : (problem_78_pre_z str_l )) (PreH8 : (hex_count_safe_78 str_l )) (PreH9 : (key_payload_safe_78 )) (PreH10 : ((string_length (str_l)) < INT_MAX)) ,
+  (GlobalStrings_missing LitMap all_key_literals_78 )
+|--
+  “ (hex_count_state_78 str_l 0 0 ) ” 
+  &&  “ (0 <= retval) ”
+  &&  (GlobalStrings_missing LitMap all_key_literals_78 )
+).
+
+Definition hex_key_entail_wit_2_split_goal_1 := 
+forall (str_l: (@list Z)) (key: Z) (retval: Z) (PreH1 : (retval = (string_length (str_l)))) (PreH2 : (0 <= ((string_length (key_payload_78)) + 1 ))) (PreH3 : (0 <= ((string_length (str_l)) + 1 ))) (PreH4 : (key = (key_ptr_78 (LitMap)))) (PreH5 : (valid_string str_l )) (PreH6 : (all_ascii str_l )) (PreH7 : (problem_78_pre_z str_l )) (PreH8 : (hex_count_safe_78 str_l )) (PreH9 : (key_payload_safe_78 )) (PreH10 : ((string_length (str_l)) < INT_MAX)) ,
+  (GlobalStrings_missing LitMap all_key_literals_78 )
+|--
+  “ (hex_count_state_78 str_l 0 0 ) ”
+.
+
+Definition hex_key_entail_wit_2_split_goal_2 := 
+forall (str_l: (@list Z)) (key: Z) (retval: Z) (PreH1 : (retval = (string_length (str_l)))) (PreH2 : (0 <= ((string_length (key_payload_78)) + 1 ))) (PreH3 : (0 <= ((string_length (str_l)) + 1 ))) (PreH4 : (key = (key_ptr_78 (LitMap)))) (PreH5 : (valid_string str_l )) (PreH6 : (all_ascii str_l )) (PreH7 : (problem_78_pre_z str_l )) (PreH8 : (hex_count_safe_78 str_l )) (PreH9 : (key_payload_safe_78 )) (PreH10 : ((string_length (str_l)) < INT_MAX)) ,
+  (GlobalStrings_missing LitMap all_key_literals_78 )
+|--
+  “ (0 <= retval) ”
+.
+
+Definition hex_key_entail_wit_2_split_goal_spatial := 
+forall (str_l: (@list Z)) (key: Z) (retval: Z) (PreH1 : (retval = (string_length (str_l)))) (PreH2 : (0 <= ((string_length (key_payload_78)) + 1 ))) (PreH3 : (0 <= ((string_length (str_l)) + 1 ))) (PreH4 : (key = (key_ptr_78 (LitMap)))) (PreH5 : (valid_string str_l )) (PreH6 : (all_ascii str_l )) (PreH7 : (problem_78_pre_z str_l )) (PreH8 : (hex_count_safe_78 str_l )) (PreH9 : (key_payload_safe_78 )) (PreH10 : ((string_length (str_l)) < INT_MAX)) ,
+  (GlobalStrings_missing LitMap all_key_literals_78 )
+|--
+  (GlobalStrings_missing LitMap all_key_literals_78 )
+.
+
+Definition hex_key_entail_wit_3 := 
+(
+forall (num_pre: Z) (str_l: (@list Z)) (out: Z) (i: Z) (n: Z) (key: Z) (retval: Z) (PreH1 : (retval <> 0)) (PreH2 : (strchr_result key_payload_78 (Znth i (c_string (str_l)) 0) retval key )) (PreH3 : (0 <= ((string_length (key_payload_78)) + 1 ))) (PreH4 : (0 <= ((string_length (str_l)) + 1 ))) (PreH5 : (i < n)) (PreH6 : (key = (key_ptr_78 (LitMap)))) (PreH7 : (n = (string_length (str_l)))) (PreH8 : (0 <= i)) (PreH9 : (i <= n)) (PreH10 : (0 <= out)) (PreH11 : (out <= i)) (PreH12 : (valid_string str_l )) (PreH13 : (all_ascii str_l )) (PreH14 : (problem_78_pre_z str_l )) (PreH15 : (hex_count_safe_78 str_l )) (PreH16 : (key_payload_safe_78 )) (PreH17 : ((string_length (str_l)) < INT_MAX)) (PreH18 : (hex_count_state_78 str_l i out )) ,
+  (store_string key key_payload_78 )
+  **  (CharArray.full num_pre ((string_length (str_l)) + 1 ) (c_string (str_l)) )
+  **  (GlobalStrings_missing LitMap all_key_literals_78 )
+|--
+  “ (key = (key_ptr_78 (LitMap))) ” 
+  &&  “ (n = (string_length (str_l))) ” 
+  &&  “ (0 <= i) ” 
+  &&  “ (i < n) ” 
+  &&  “ (0 <= (out + 1 )) ” 
+  &&  “ ((out + 1 ) <= (i + 1 )) ” 
+  &&  “ (0 <= (Znth i (c_string (str_l)) 0)) ” 
+  &&  “ ((Znth i (c_string (str_l)) 0) <= 127) ” 
+  &&  “ (valid_string str_l ) ” 
+  &&  “ (all_ascii str_l ) ” 
+  &&  “ (problem_78_pre_z str_l ) ” 
+  &&  “ (hex_count_safe_78 str_l ) ” 
+  &&  “ (key_payload_safe_78 ) ” 
+  &&  “ ((string_length (str_l)) < INT_MAX) ” 
+  &&  “ (hex_hit_step_78 str_l i (out + 1 ) ) ” 
+  &&  “ (hex_count_state_78 str_l (i + 1 ) (out + 1 ) ) ”
+  &&  (store_string num_pre str_l )
+  **  (store_string key key_payload_78 )
+  **  (GlobalStrings_missing LitMap all_key_literals_78 )
+) \/
+(
+forall (str_l: (@list Z)) (out: Z) (i: Z) (n: Z) (key: Z) (retval: Z) (PreH1 : (retval <> 0)) (PreH2 : (strchr_result key_payload_78 (Znth i (c_string (str_l)) 0) retval key )) (PreH3 : (0 <= ((string_length (key_payload_78)) + 1 ))) (PreH4 : (0 <= ((string_length (str_l)) + 1 ))) (PreH5 : (i < n)) (PreH6 : (key = (key_ptr_78 (LitMap)))) (PreH7 : (n = (string_length (str_l)))) (PreH8 : (0 <= i)) (PreH9 : (i <= n)) (PreH10 : (0 <= out)) (PreH11 : (out <= i)) (PreH12 : (valid_string str_l )) (PreH13 : (all_ascii str_l )) (PreH14 : (problem_78_pre_z str_l )) (PreH15 : (hex_count_safe_78 str_l )) (PreH16 : (key_payload_safe_78 )) (PreH17 : ((string_length (str_l)) < INT_MAX)) (PreH18 : (hex_count_state_78 str_l i out )) ,
+  (GlobalStrings_missing LitMap all_key_literals_78 )
+|--
+  “ (hex_count_state_78 str_l (i + 1 ) (out + 1 ) ) ” 
+  &&  “ (hex_hit_step_78 str_l i (out + 1 ) ) ” 
+  &&  “ ((Znth i (c_string (str_l)) 0) <= 127) ” 
+  &&  “ (0 <= (Znth i (c_string (str_l)) 0)) ”
+  &&  (GlobalStrings_missing LitMap all_key_literals_78 )
+).
+
+Definition hex_key_entail_wit_3_split_goal_1 := 
+forall (str_l: (@list Z)) (out: Z) (i: Z) (n: Z) (key: Z) (retval: Z) (PreH1 : (retval <> 0)) (PreH2 : (strchr_result key_payload_78 (Znth i (c_string (str_l)) 0) retval key )) (PreH3 : (0 <= ((string_length (key_payload_78)) + 1 ))) (PreH4 : (0 <= ((string_length (str_l)) + 1 ))) (PreH5 : (i < n)) (PreH6 : (key = (key_ptr_78 (LitMap)))) (PreH7 : (n = (string_length (str_l)))) (PreH8 : (0 <= i)) (PreH9 : (i <= n)) (PreH10 : (0 <= out)) (PreH11 : (out <= i)) (PreH12 : (valid_string str_l )) (PreH13 : (all_ascii str_l )) (PreH14 : (problem_78_pre_z str_l )) (PreH15 : (hex_count_safe_78 str_l )) (PreH16 : (key_payload_safe_78 )) (PreH17 : ((string_length (str_l)) < INT_MAX)) (PreH18 : (hex_count_state_78 str_l i out )) ,
+  (GlobalStrings_missing LitMap all_key_literals_78 )
+|--
+  “ (hex_count_state_78 str_l (i + 1 ) (out + 1 ) ) ”
+.
+
+Definition hex_key_entail_wit_3_split_goal_2 := 
+forall (str_l: (@list Z)) (out: Z) (i: Z) (n: Z) (key: Z) (retval: Z) (PreH1 : (retval <> 0)) (PreH2 : (strchr_result key_payload_78 (Znth i (c_string (str_l)) 0) retval key )) (PreH3 : (0 <= ((string_length (key_payload_78)) + 1 ))) (PreH4 : (0 <= ((string_length (str_l)) + 1 ))) (PreH5 : (i < n)) (PreH6 : (key = (key_ptr_78 (LitMap)))) (PreH7 : (n = (string_length (str_l)))) (PreH8 : (0 <= i)) (PreH9 : (i <= n)) (PreH10 : (0 <= out)) (PreH11 : (out <= i)) (PreH12 : (valid_string str_l )) (PreH13 : (all_ascii str_l )) (PreH14 : (problem_78_pre_z str_l )) (PreH15 : (hex_count_safe_78 str_l )) (PreH16 : (key_payload_safe_78 )) (PreH17 : ((string_length (str_l)) < INT_MAX)) (PreH18 : (hex_count_state_78 str_l i out )) ,
+  (GlobalStrings_missing LitMap all_key_literals_78 )
+|--
+  “ (hex_hit_step_78 str_l i (out + 1 ) ) ”
+.
+
+Definition hex_key_entail_wit_3_split_goal_3 := 
+forall (str_l: (@list Z)) (out: Z) (i: Z) (n: Z) (key: Z) (retval: Z) (PreH1 : (retval <> 0)) (PreH2 : (strchr_result key_payload_78 (Znth i (c_string (str_l)) 0) retval key )) (PreH3 : (0 <= ((string_length (key_payload_78)) + 1 ))) (PreH4 : (0 <= ((string_length (str_l)) + 1 ))) (PreH5 : (i < n)) (PreH6 : (key = (key_ptr_78 (LitMap)))) (PreH7 : (n = (string_length (str_l)))) (PreH8 : (0 <= i)) (PreH9 : (i <= n)) (PreH10 : (0 <= out)) (PreH11 : (out <= i)) (PreH12 : (valid_string str_l )) (PreH13 : (all_ascii str_l )) (PreH14 : (problem_78_pre_z str_l )) (PreH15 : (hex_count_safe_78 str_l )) (PreH16 : (key_payload_safe_78 )) (PreH17 : ((string_length (str_l)) < INT_MAX)) (PreH18 : (hex_count_state_78 str_l i out )) ,
+  (GlobalStrings_missing LitMap all_key_literals_78 )
+|--
+  “ ((Znth i (c_string (str_l)) 0) <= 127) ”
+.
+
+Definition hex_key_entail_wit_3_split_goal_4 := 
+forall (str_l: (@list Z)) (out: Z) (i: Z) (n: Z) (key: Z) (retval: Z) (PreH1 : (retval <> 0)) (PreH2 : (strchr_result key_payload_78 (Znth i (c_string (str_l)) 0) retval key )) (PreH3 : (0 <= ((string_length (key_payload_78)) + 1 ))) (PreH4 : (0 <= ((string_length (str_l)) + 1 ))) (PreH5 : (i < n)) (PreH6 : (key = (key_ptr_78 (LitMap)))) (PreH7 : (n = (string_length (str_l)))) (PreH8 : (0 <= i)) (PreH9 : (i <= n)) (PreH10 : (0 <= out)) (PreH11 : (out <= i)) (PreH12 : (valid_string str_l )) (PreH13 : (all_ascii str_l )) (PreH14 : (problem_78_pre_z str_l )) (PreH15 : (hex_count_safe_78 str_l )) (PreH16 : (key_payload_safe_78 )) (PreH17 : ((string_length (str_l)) < INT_MAX)) (PreH18 : (hex_count_state_78 str_l i out )) ,
+  (GlobalStrings_missing LitMap all_key_literals_78 )
+|--
+  “ (0 <= (Znth i (c_string (str_l)) 0)) ”
+.
+
+Definition hex_key_entail_wit_3_split_goal_spatial := 
+forall (str_l: (@list Z)) (out: Z) (i: Z) (n: Z) (key: Z) (retval: Z) (PreH1 : (retval <> 0)) (PreH2 : (strchr_result key_payload_78 (Znth i (c_string (str_l)) 0) retval key )) (PreH3 : (0 <= ((string_length (key_payload_78)) + 1 ))) (PreH4 : (0 <= ((string_length (str_l)) + 1 ))) (PreH5 : (i < n)) (PreH6 : (key = (key_ptr_78 (LitMap)))) (PreH7 : (n = (string_length (str_l)))) (PreH8 : (0 <= i)) (PreH9 : (i <= n)) (PreH10 : (0 <= out)) (PreH11 : (out <= i)) (PreH12 : (valid_string str_l )) (PreH13 : (all_ascii str_l )) (PreH14 : (problem_78_pre_z str_l )) (PreH15 : (hex_count_safe_78 str_l )) (PreH16 : (key_payload_safe_78 )) (PreH17 : ((string_length (str_l)) < INT_MAX)) (PreH18 : (hex_count_state_78 str_l i out )) ,
+  (GlobalStrings_missing LitMap all_key_literals_78 )
+|--
+  (GlobalStrings_missing LitMap all_key_literals_78 )
+.
+
+Definition hex_key_entail_wit_4 := 
+(
+forall (num_pre: Z) (str_l: (@list Z)) (out: Z) (i: Z) (n: Z) (key: Z) (retval: Z) (PreH1 : (retval = 0)) (PreH2 : (strchr_result key_payload_78 (Znth i (c_string (str_l)) 0) retval key )) (PreH3 : (0 <= ((string_length (key_payload_78)) + 1 ))) (PreH4 : (0 <= ((string_length (str_l)) + 1 ))) (PreH5 : (i < n)) (PreH6 : (key = (key_ptr_78 (LitMap)))) (PreH7 : (n = (string_length (str_l)))) (PreH8 : (0 <= i)) (PreH9 : (i <= n)) (PreH10 : (0 <= out)) (PreH11 : (out <= i)) (PreH12 : (valid_string str_l )) (PreH13 : (all_ascii str_l )) (PreH14 : (problem_78_pre_z str_l )) (PreH15 : (hex_count_safe_78 str_l )) (PreH16 : (key_payload_safe_78 )) (PreH17 : ((string_length (str_l)) < INT_MAX)) (PreH18 : (hex_count_state_78 str_l i out )) ,
+  (store_string key key_payload_78 )
+  **  (CharArray.full num_pre ((string_length (str_l)) + 1 ) (c_string (str_l)) )
+  **  (GlobalStrings_missing LitMap all_key_literals_78 )
+|--
+  “ (key = (key_ptr_78 (LitMap))) ” 
+  &&  “ (n = (string_length (str_l))) ” 
+  &&  “ (0 <= i) ” 
+  &&  “ (i < n) ” 
+  &&  “ (0 <= out) ” 
+  &&  “ (out <= i) ” 
+  &&  “ (0 <= (Znth i (c_string (str_l)) 0)) ” 
+  &&  “ ((Znth i (c_string (str_l)) 0) <= 127) ” 
+  &&  “ (valid_string str_l ) ” 
+  &&  “ (all_ascii str_l ) ” 
+  &&  “ (problem_78_pre_z str_l ) ” 
+  &&  “ (hex_count_safe_78 str_l ) ” 
+  &&  “ (key_payload_safe_78 ) ” 
+  &&  “ ((string_length (str_l)) < INT_MAX) ” 
+  &&  “ (hex_miss_step_78 str_l i out ) ” 
+  &&  “ (hex_count_state_78 str_l (i + 1 ) out ) ”
+  &&  (store_string num_pre str_l )
+  **  (store_string key key_payload_78 )
+  **  (GlobalStrings_missing LitMap all_key_literals_78 )
+) \/
+(
+forall (str_l: (@list Z)) (out: Z) (i: Z) (n: Z) (key: Z) (retval: Z) (PreH1 : (retval = 0)) (PreH2 : (strchr_result key_payload_78 (Znth i (c_string (str_l)) 0) retval key )) (PreH3 : (0 <= ((string_length (key_payload_78)) + 1 ))) (PreH4 : (0 <= ((string_length (str_l)) + 1 ))) (PreH5 : (i < n)) (PreH6 : (key = (key_ptr_78 (LitMap)))) (PreH7 : (n = (string_length (str_l)))) (PreH8 : (0 <= i)) (PreH9 : (i <= n)) (PreH10 : (0 <= out)) (PreH11 : (out <= i)) (PreH12 : (valid_string str_l )) (PreH13 : (all_ascii str_l )) (PreH14 : (problem_78_pre_z str_l )) (PreH15 : (hex_count_safe_78 str_l )) (PreH16 : (key_payload_safe_78 )) (PreH17 : ((string_length (str_l)) < INT_MAX)) (PreH18 : (hex_count_state_78 str_l i out )) ,
+  (GlobalStrings_missing LitMap all_key_literals_78 )
+|--
+  “ (hex_count_state_78 str_l (i + 1 ) out ) ” 
+  &&  “ (hex_miss_step_78 str_l i out ) ” 
+  &&  “ ((Znth i (c_string (str_l)) 0) <= 127) ” 
+  &&  “ (0 <= (Znth i (c_string (str_l)) 0)) ”
+  &&  (GlobalStrings_missing LitMap all_key_literals_78 )
+).
+
+Definition hex_key_entail_wit_4_split_goal_1 := 
+forall (str_l: (@list Z)) (out: Z) (i: Z) (n: Z) (key: Z) (retval: Z) (PreH1 : (retval = 0)) (PreH2 : (strchr_result key_payload_78 (Znth i (c_string (str_l)) 0) retval key )) (PreH3 : (0 <= ((string_length (key_payload_78)) + 1 ))) (PreH4 : (0 <= ((string_length (str_l)) + 1 ))) (PreH5 : (i < n)) (PreH6 : (key = (key_ptr_78 (LitMap)))) (PreH7 : (n = (string_length (str_l)))) (PreH8 : (0 <= i)) (PreH9 : (i <= n)) (PreH10 : (0 <= out)) (PreH11 : (out <= i)) (PreH12 : (valid_string str_l )) (PreH13 : (all_ascii str_l )) (PreH14 : (problem_78_pre_z str_l )) (PreH15 : (hex_count_safe_78 str_l )) (PreH16 : (key_payload_safe_78 )) (PreH17 : ((string_length (str_l)) < INT_MAX)) (PreH18 : (hex_count_state_78 str_l i out )) ,
+  (GlobalStrings_missing LitMap all_key_literals_78 )
+|--
+  “ (hex_count_state_78 str_l (i + 1 ) out ) ”
+.
+
+Definition hex_key_entail_wit_4_split_goal_2 := 
+forall (str_l: (@list Z)) (out: Z) (i: Z) (n: Z) (key: Z) (retval: Z) (PreH1 : (retval = 0)) (PreH2 : (strchr_result key_payload_78 (Znth i (c_string (str_l)) 0) retval key )) (PreH3 : (0 <= ((string_length (key_payload_78)) + 1 ))) (PreH4 : (0 <= ((string_length (str_l)) + 1 ))) (PreH5 : (i < n)) (PreH6 : (key = (key_ptr_78 (LitMap)))) (PreH7 : (n = (string_length (str_l)))) (PreH8 : (0 <= i)) (PreH9 : (i <= n)) (PreH10 : (0 <= out)) (PreH11 : (out <= i)) (PreH12 : (valid_string str_l )) (PreH13 : (all_ascii str_l )) (PreH14 : (problem_78_pre_z str_l )) (PreH15 : (hex_count_safe_78 str_l )) (PreH16 : (key_payload_safe_78 )) (PreH17 : ((string_length (str_l)) < INT_MAX)) (PreH18 : (hex_count_state_78 str_l i out )) ,
+  (GlobalStrings_missing LitMap all_key_literals_78 )
+|--
+  “ (hex_miss_step_78 str_l i out ) ”
+.
+
+Definition hex_key_entail_wit_4_split_goal_3 := 
+forall (str_l: (@list Z)) (out: Z) (i: Z) (n: Z) (key: Z) (retval: Z) (PreH1 : (retval = 0)) (PreH2 : (strchr_result key_payload_78 (Znth i (c_string (str_l)) 0) retval key )) (PreH3 : (0 <= ((string_length (key_payload_78)) + 1 ))) (PreH4 : (0 <= ((string_length (str_l)) + 1 ))) (PreH5 : (i < n)) (PreH6 : (key = (key_ptr_78 (LitMap)))) (PreH7 : (n = (string_length (str_l)))) (PreH8 : (0 <= i)) (PreH9 : (i <= n)) (PreH10 : (0 <= out)) (PreH11 : (out <= i)) (PreH12 : (valid_string str_l )) (PreH13 : (all_ascii str_l )) (PreH14 : (problem_78_pre_z str_l )) (PreH15 : (hex_count_safe_78 str_l )) (PreH16 : (key_payload_safe_78 )) (PreH17 : ((string_length (str_l)) < INT_MAX)) (PreH18 : (hex_count_state_78 str_l i out )) ,
+  (GlobalStrings_missing LitMap all_key_literals_78 )
+|--
+  “ ((Znth i (c_string (str_l)) 0) <= 127) ”
+.
+
+Definition hex_key_entail_wit_4_split_goal_4 := 
+forall (str_l: (@list Z)) (out: Z) (i: Z) (n: Z) (key: Z) (retval: Z) (PreH1 : (retval = 0)) (PreH2 : (strchr_result key_payload_78 (Znth i (c_string (str_l)) 0) retval key )) (PreH3 : (0 <= ((string_length (key_payload_78)) + 1 ))) (PreH4 : (0 <= ((string_length (str_l)) + 1 ))) (PreH5 : (i < n)) (PreH6 : (key = (key_ptr_78 (LitMap)))) (PreH7 : (n = (string_length (str_l)))) (PreH8 : (0 <= i)) (PreH9 : (i <= n)) (PreH10 : (0 <= out)) (PreH11 : (out <= i)) (PreH12 : (valid_string str_l )) (PreH13 : (all_ascii str_l )) (PreH14 : (problem_78_pre_z str_l )) (PreH15 : (hex_count_safe_78 str_l )) (PreH16 : (key_payload_safe_78 )) (PreH17 : ((string_length (str_l)) < INT_MAX)) (PreH18 : (hex_count_state_78 str_l i out )) ,
+  (GlobalStrings_missing LitMap all_key_literals_78 )
+|--
+  “ (0 <= (Znth i (c_string (str_l)) 0)) ”
+.
+
+Definition hex_key_entail_wit_4_split_goal_spatial := 
+forall (str_l: (@list Z)) (out: Z) (i: Z) (n: Z) (key: Z) (retval: Z) (PreH1 : (retval = 0)) (PreH2 : (strchr_result key_payload_78 (Znth i (c_string (str_l)) 0) retval key )) (PreH3 : (0 <= ((string_length (key_payload_78)) + 1 ))) (PreH4 : (0 <= ((string_length (str_l)) + 1 ))) (PreH5 : (i < n)) (PreH6 : (key = (key_ptr_78 (LitMap)))) (PreH7 : (n = (string_length (str_l)))) (PreH8 : (0 <= i)) (PreH9 : (i <= n)) (PreH10 : (0 <= out)) (PreH11 : (out <= i)) (PreH12 : (valid_string str_l )) (PreH13 : (all_ascii str_l )) (PreH14 : (problem_78_pre_z str_l )) (PreH15 : (hex_count_safe_78 str_l )) (PreH16 : (key_payload_safe_78 )) (PreH17 : ((string_length (str_l)) < INT_MAX)) (PreH18 : (hex_count_state_78 str_l i out )) ,
+  (GlobalStrings_missing LitMap all_key_literals_78 )
+|--
+  (GlobalStrings_missing LitMap all_key_literals_78 )
+.
+
+Definition hex_key_entail_wit_5_1 := 
+forall (num_pre: Z) (str_l: (@list Z)) (key: Z) (n: Z) (i: Z) (out: Z) (ch: Z) (PreH1 : (key = (key_ptr_78 (LitMap)))) (PreH2 : (n = (string_length (str_l)))) (PreH3 : (0 <= i)) (PreH4 : (i < n)) (PreH5 : (0 <= out)) (PreH6 : (out <= (i + 1 ))) (PreH7 : (0 <= ch)) (PreH8 : (ch <= 127)) (PreH9 : (valid_string str_l )) (PreH10 : (all_ascii str_l )) (PreH11 : (problem_78_pre_z str_l )) (PreH12 : (hex_count_safe_78 str_l )) (PreH13 : (key_payload_safe_78 )) (PreH14 : ((string_length (str_l)) < INT_MAX)) (PreH15 : (hex_hit_step_78 str_l i out )) (PreH16 : (hex_count_state_78 str_l (i + 1 ) out )) ,
+  (store_string num_pre str_l )
+  **  (store_string key key_payload_78 )
+  **  (GlobalStrings_missing LitMap all_key_literals_78 )
+|--
+  “ (key = (key_ptr_78 (LitMap))) ” 
+  &&  “ (n = (string_length (str_l))) ” 
+  &&  “ (0 <= (i + 1 )) ” 
+  &&  “ ((i + 1 ) <= n) ” 
+  &&  “ (0 <= out) ” 
+  &&  “ (out <= (i + 1 )) ” 
+  &&  “ (valid_string str_l ) ” 
+  &&  “ (all_ascii str_l ) ” 
+  &&  “ (problem_78_pre_z str_l ) ” 
+  &&  “ (hex_count_safe_78 str_l ) ” 
+  &&  “ (key_payload_safe_78 ) ” 
+  &&  “ ((string_length (str_l)) < INT_MAX) ” 
+  &&  “ (hex_count_state_78 str_l (i + 1 ) out ) ”
+  &&  (store_string num_pre str_l )
+  **  (store_string key key_payload_78 )
+  **  (GlobalStrings_missing LitMap all_key_literals_78 )
+.
+
+Definition hex_key_entail_wit_5_2 := 
+forall (num_pre: Z) (str_l: (@list Z)) (key: Z) (n: Z) (i: Z) (out: Z) (ch: Z) (PreH1 : (key = (key_ptr_78 (LitMap)))) (PreH2 : (n = (string_length (str_l)))) (PreH3 : (0 <= i)) (PreH4 : (i < n)) (PreH5 : (0 <= out)) (PreH6 : (out <= i)) (PreH7 : (0 <= ch)) (PreH8 : (ch <= 127)) (PreH9 : (valid_string str_l )) (PreH10 : (all_ascii str_l )) (PreH11 : (problem_78_pre_z str_l )) (PreH12 : (hex_count_safe_78 str_l )) (PreH13 : (key_payload_safe_78 )) (PreH14 : ((string_length (str_l)) < INT_MAX)) (PreH15 : (hex_miss_step_78 str_l i out )) (PreH16 : (hex_count_state_78 str_l (i + 1 ) out )) ,
+  (store_string num_pre str_l )
+  **  (store_string key key_payload_78 )
+  **  (GlobalStrings_missing LitMap all_key_literals_78 )
+|--
+  “ (key = (key_ptr_78 (LitMap))) ” 
+  &&  “ (n = (string_length (str_l))) ” 
+  &&  “ (0 <= (i + 1 )) ” 
+  &&  “ ((i + 1 ) <= n) ” 
+  &&  “ (0 <= out) ” 
+  &&  “ (out <= (i + 1 )) ” 
+  &&  “ (valid_string str_l ) ” 
+  &&  “ (all_ascii str_l ) ” 
+  &&  “ (problem_78_pre_z str_l ) ” 
+  &&  “ (hex_count_safe_78 str_l ) ” 
+  &&  “ (key_payload_safe_78 ) ” 
+  &&  “ ((string_length (str_l)) < INT_MAX) ” 
+  &&  “ (hex_count_state_78 str_l (i + 1 ) out ) ”
+  &&  (store_string num_pre str_l )
+  **  (store_string key key_payload_78 )
+  **  (GlobalStrings_missing LitMap all_key_literals_78 )
+.
+
+Definition hex_key_entail_wit_6 := 
+(
+forall (num_pre: Z) (str_l: (@list Z)) (out: Z) (i: Z) (n: Z) (key: Z) (PreH1 : (i >= n)) (PreH2 : (key = (key_ptr_78 (LitMap)))) (PreH3 : (n = (string_length (str_l)))) (PreH4 : (0 <= i)) (PreH5 : (i <= n)) (PreH6 : (0 <= out)) (PreH7 : (out <= i)) (PreH8 : (valid_string str_l )) (PreH9 : (all_ascii str_l )) (PreH10 : (problem_78_pre_z str_l )) (PreH11 : (hex_count_safe_78 str_l )) (PreH12 : (key_payload_safe_78 )) (PreH13 : ((string_length (str_l)) < INT_MAX)) (PreH14 : (hex_count_state_78 str_l i out )) ,
+  (store_string num_pre str_l )
+  **  (store_string key key_payload_78 )
+  **  (GlobalStrings_missing LitMap all_key_literals_78 )
+|--
+  “ (key = (key_ptr_78 (LitMap))) ” 
+  &&  “ (n = (string_length (str_l))) ” 
+  &&  “ (0 <= out) ” 
+  &&  “ (out <= n) ” 
+  &&  “ (valid_string str_l ) ” 
+  &&  “ (all_ascii str_l ) ” 
+  &&  “ (problem_78_pre_z str_l ) ” 
+  &&  “ (hex_count_safe_78 str_l ) ” 
+  &&  “ (key_payload_safe_78 ) ” 
+  &&  “ ((string_length (str_l)) < INT_MAX) ” 
+  &&  “ (hex_count_state_78 str_l n out ) ” 
+  &&  “ (hex_final_78 str_l out ) ” 
+  &&  “ (problem_78_spec_z str_l out ) ”
+  &&  (store_string num_pre str_l )
+  **  (store_string key key_payload_78 )
+  **  (GlobalStrings_missing LitMap all_key_literals_78 )
+) \/
+(
+forall (str_l: (@list Z)) (out: Z) (i: Z) (n: Z) (key: Z) (PreH1 : (0 <= ((string_length (key_payload_78)) + 1 ))) (PreH2 : (0 <= ((string_length (str_l)) + 1 ))) (PreH3 : (i >= n)) (PreH4 : (key = (key_ptr_78 (LitMap)))) (PreH5 : (n = (string_length (str_l)))) (PreH6 : (0 <= i)) (PreH7 : (i <= n)) (PreH8 : (0 <= out)) (PreH9 : (out <= i)) (PreH10 : (valid_string str_l )) (PreH11 : (all_ascii str_l )) (PreH12 : (problem_78_pre_z str_l )) (PreH13 : (hex_count_safe_78 str_l )) (PreH14 : (key_payload_safe_78 )) (PreH15 : ((string_length (str_l)) < INT_MAX)) (PreH16 : (hex_count_state_78 str_l i out )) ,
+  (GlobalStrings_missing LitMap all_key_literals_78 )
+|--
+  “ (problem_78_spec_z str_l out ) ” 
+  &&  “ (hex_final_78 str_l out ) ” 
+  &&  “ (hex_count_state_78 str_l n out ) ”
+  &&  (GlobalStrings_missing LitMap all_key_literals_78 )
+).
+
+Definition hex_key_entail_wit_6_split_goal_1 := 
+forall (str_l: (@list Z)) (out: Z) (i: Z) (n: Z) (key: Z) (PreH1 : (0 <= ((string_length (key_payload_78)) + 1 ))) (PreH2 : (0 <= ((string_length (str_l)) + 1 ))) (PreH3 : (i >= n)) (PreH4 : (key = (key_ptr_78 (LitMap)))) (PreH5 : (n = (string_length (str_l)))) (PreH6 : (0 <= i)) (PreH7 : (i <= n)) (PreH8 : (0 <= out)) (PreH9 : (out <= i)) (PreH10 : (valid_string str_l )) (PreH11 : (all_ascii str_l )) (PreH12 : (problem_78_pre_z str_l )) (PreH13 : (hex_count_safe_78 str_l )) (PreH14 : (key_payload_safe_78 )) (PreH15 : ((string_length (str_l)) < INT_MAX)) (PreH16 : (hex_count_state_78 str_l i out )) ,
+  (GlobalStrings_missing LitMap all_key_literals_78 )
+|--
+  “ (problem_78_spec_z str_l out ) ”
+.
+
+Definition hex_key_entail_wit_6_split_goal_2 := 
+forall (str_l: (@list Z)) (out: Z) (i: Z) (n: Z) (key: Z) (PreH1 : (0 <= ((string_length (key_payload_78)) + 1 ))) (PreH2 : (0 <= ((string_length (str_l)) + 1 ))) (PreH3 : (i >= n)) (PreH4 : (key = (key_ptr_78 (LitMap)))) (PreH5 : (n = (string_length (str_l)))) (PreH6 : (0 <= i)) (PreH7 : (i <= n)) (PreH8 : (0 <= out)) (PreH9 : (out <= i)) (PreH10 : (valid_string str_l )) (PreH11 : (all_ascii str_l )) (PreH12 : (problem_78_pre_z str_l )) (PreH13 : (hex_count_safe_78 str_l )) (PreH14 : (key_payload_safe_78 )) (PreH15 : ((string_length (str_l)) < INT_MAX)) (PreH16 : (hex_count_state_78 str_l i out )) ,
+  (GlobalStrings_missing LitMap all_key_literals_78 )
+|--
+  “ (hex_final_78 str_l out ) ”
+.
+
+Definition hex_key_entail_wit_6_split_goal_3 := 
+forall (str_l: (@list Z)) (out: Z) (i: Z) (n: Z) (key: Z) (PreH1 : (0 <= ((string_length (key_payload_78)) + 1 ))) (PreH2 : (0 <= ((string_length (str_l)) + 1 ))) (PreH3 : (i >= n)) (PreH4 : (key = (key_ptr_78 (LitMap)))) (PreH5 : (n = (string_length (str_l)))) (PreH6 : (0 <= i)) (PreH7 : (i <= n)) (PreH8 : (0 <= out)) (PreH9 : (out <= i)) (PreH10 : (valid_string str_l )) (PreH11 : (all_ascii str_l )) (PreH12 : (problem_78_pre_z str_l )) (PreH13 : (hex_count_safe_78 str_l )) (PreH14 : (key_payload_safe_78 )) (PreH15 : ((string_length (str_l)) < INT_MAX)) (PreH16 : (hex_count_state_78 str_l i out )) ,
+  (GlobalStrings_missing LitMap all_key_literals_78 )
+|--
+  “ (hex_count_state_78 str_l n out ) ”
+.
+
+Definition hex_key_entail_wit_6_split_goal_spatial := 
+forall (str_l: (@list Z)) (out: Z) (i: Z) (n: Z) (key: Z) (PreH1 : (0 <= ((string_length (key_payload_78)) + 1 ))) (PreH2 : (0 <= ((string_length (str_l)) + 1 ))) (PreH3 : (i >= n)) (PreH4 : (key = (key_ptr_78 (LitMap)))) (PreH5 : (n = (string_length (str_l)))) (PreH6 : (0 <= i)) (PreH7 : (i <= n)) (PreH8 : (0 <= out)) (PreH9 : (out <= i)) (PreH10 : (valid_string str_l )) (PreH11 : (all_ascii str_l )) (PreH12 : (problem_78_pre_z str_l )) (PreH13 : (hex_count_safe_78 str_l )) (PreH14 : (key_payload_safe_78 )) (PreH15 : ((string_length (str_l)) < INT_MAX)) (PreH16 : (hex_count_state_78 str_l i out )) ,
+  (GlobalStrings_missing LitMap all_key_literals_78 )
+|--
+  (GlobalStrings_missing LitMap all_key_literals_78 )
+.
+
+Definition hex_key_return_wit_1 := 
+(
+forall (num_pre: Z) (str_l: (@list Z)) (key: Z) (n: Z) (out: Z) (PreH1 : (key = (key_ptr_78 (LitMap)))) (PreH2 : (n = (string_length (str_l)))) (PreH3 : (0 <= out)) (PreH4 : (out <= n)) (PreH5 : (valid_string str_l )) (PreH6 : (all_ascii str_l )) (PreH7 : (problem_78_pre_z str_l )) (PreH8 : (hex_count_safe_78 str_l )) (PreH9 : (key_payload_safe_78 )) (PreH10 : ((string_length (str_l)) < INT_MAX)) (PreH11 : (hex_count_state_78 str_l n out )) (PreH12 : (hex_final_78 str_l out )) (PreH13 : (problem_78_spec_z str_l out )) ,
+  (store_string num_pre str_l )
+  **  (store_string key key_payload_78 )
+  **  (GlobalStrings_missing LitMap all_key_literals_78 )
+|--
+  “ (problem_78_spec_z str_l out ) ”
+  &&  (store_string num_pre str_l )
+  **  (store_string (key_ptr_78 (LitMap)) key_payload_78 )
+  **  (GlobalStrings_missing LitMap all_key_literals_78 )
+) \/
+(
+forall (str_l: (@list Z)) (key: Z) (n: Z) (out: Z) (PreH1 : (0 <= ((string_length (key_payload_78)) + 1 ))) (PreH2 : (0 <= ((string_length (str_l)) + 1 ))) (PreH3 : (key = (key_ptr_78 (LitMap)))) (PreH4 : (n = (string_length (str_l)))) (PreH5 : (0 <= out)) (PreH6 : (out <= n)) (PreH7 : (valid_string str_l )) (PreH8 : (all_ascii str_l )) (PreH9 : (problem_78_pre_z str_l )) (PreH10 : (hex_count_safe_78 str_l )) (PreH11 : (key_payload_safe_78 )) (PreH12 : ((string_length (str_l)) < INT_MAX)) (PreH13 : (hex_count_state_78 str_l n out )) (PreH14 : (hex_final_78 str_l out )) (PreH15 : (problem_78_spec_z str_l out )) ,
+  (CharArray.full key ((string_length (key_payload_78)) + 1 ) (c_string (key_payload_78)) )
+  **  (GlobalStrings_missing LitMap all_key_literals_78 )
+|--
+  (CharArray.full (key_ptr_78 (LitMap)) ((string_length (key_payload_78)) + 1 ) (c_string (key_payload_78)) )
+  **  (GlobalStrings_missing LitMap all_key_literals_78 )
+).
+
+Definition hex_key_return_wit_1_split_goal_spatial := 
+forall (str_l: (@list Z)) (key: Z) (n: Z) (out: Z) (PreH1 : (0 <= ((string_length (key_payload_78)) + 1 ))) (PreH2 : (0 <= ((string_length (str_l)) + 1 ))) (PreH3 : (key = (key_ptr_78 (LitMap)))) (PreH4 : (n = (string_length (str_l)))) (PreH5 : (0 <= out)) (PreH6 : (out <= n)) (PreH7 : (valid_string str_l )) (PreH8 : (all_ascii str_l )) (PreH9 : (problem_78_pre_z str_l )) (PreH10 : (hex_count_safe_78 str_l )) (PreH11 : (key_payload_safe_78 )) (PreH12 : ((string_length (str_l)) < INT_MAX)) (PreH13 : (hex_count_state_78 str_l n out )) (PreH14 : (hex_final_78 str_l out )) (PreH15 : (problem_78_spec_z str_l out )) ,
+  (CharArray.full key ((string_length (key_payload_78)) + 1 ) (c_string (key_payload_78)) )
+  **  (GlobalStrings_missing LitMap all_key_literals_78 )
+|--
+  (CharArray.full (key_ptr_78 (LitMap)) ((string_length (key_payload_78)) + 1 ) (c_string (key_payload_78)) )
+  **  (GlobalStrings_missing LitMap all_key_literals_78 )
+.
+
+Definition hex_key_partial_solve_wit_1_pure := 
+forall (num_pre: Z) (str_l: (@list Z)) (key: Z) (PreH1 : (key = (key_ptr_78 (LitMap)))) (PreH2 : (valid_string str_l )) (PreH3 : (all_ascii str_l )) (PreH4 : (problem_78_pre_z str_l )) (PreH5 : (hex_count_safe_78 str_l )) (PreH6 : (key_payload_safe_78 )) (PreH7 : ((string_length (str_l)) < INT_MAX)) ,
+  ((( &( "n" ) )) # Int  |->_)
+  **  ((( &( "num" ) )) # Ptr  |-> num_pre)
+  **  ((( &( "key" ) )) # Ptr  |-> key)
+  **  (store_string num_pre str_l )
+  **  (store_string key key_payload_78 )
+  **  (GlobalStrings_missing LitMap all_key_literals_78 )
+|--
+  “ (valid_string str_l ) ” 
+  &&  “ ((string_length (str_l)) < INT_MAX) ”
+.
+
+Definition hex_key_partial_solve_wit_1_aux := 
+forall (num_pre: Z) (str_l: (@list Z)) (key: Z) (PreH1 : (key = (key_ptr_78 (LitMap)))) (PreH2 : (valid_string str_l )) (PreH3 : (all_ascii str_l )) (PreH4 : (problem_78_pre_z str_l )) (PreH5 : (hex_count_safe_78 str_l )) (PreH6 : (key_payload_safe_78 )) (PreH7 : ((string_length (str_l)) < INT_MAX)) ,
+  (store_string num_pre str_l )
+  **  (store_string key key_payload_78 )
+  **  (GlobalStrings_missing LitMap all_key_literals_78 )
+|--
+  “ (valid_string str_l ) ” 
+  &&  “ ((string_length (str_l)) < INT_MAX) ” 
+  &&  “ (0 <= ((string_length (key_payload_78)) + 1 )) ” 
+  &&  “ (0 <= ((string_length (str_l)) + 1 )) ” 
+  &&  “ (key = (key_ptr_78 (LitMap))) ” 
+  &&  “ (valid_string str_l ) ” 
+  &&  “ (all_ascii str_l ) ” 
+  &&  “ (problem_78_pre_z str_l ) ” 
+  &&  “ (hex_count_safe_78 str_l ) ” 
+  &&  “ (key_payload_safe_78 ) ” 
+  &&  “ ((string_length (str_l)) < INT_MAX) ”
+  &&  (store_string num_pre str_l )
+  **  (CharArray.full key ((string_length (key_payload_78)) + 1 ) (c_string (key_payload_78)) )
+  **  (GlobalStrings_missing LitMap all_key_literals_78 )
+.
+
+Definition hex_key_partial_solve_wit_1 := hex_key_partial_solve_wit_1_pure -> hex_key_partial_solve_wit_1_aux.
+
+Definition hex_key_partial_solve_wit_2_pure := 
+(
+forall (num_pre: Z) (str_l: (@list Z)) (out: Z) (i: Z) (n: Z) (key: Z) (PreH1 : (i < n)) (PreH2 : (key = (key_ptr_78 (LitMap)))) (PreH3 : (n = (string_length (str_l)))) (PreH4 : (0 <= i)) (PreH5 : (i <= n)) (PreH6 : (0 <= out)) (PreH7 : (out <= i)) (PreH8 : (valid_string str_l )) (PreH9 : (all_ascii str_l )) (PreH10 : (problem_78_pre_z str_l )) (PreH11 : (hex_count_safe_78 str_l )) (PreH12 : (key_payload_safe_78 )) (PreH13 : ((string_length (str_l)) < INT_MAX)) (PreH14 : (hex_count_state_78 str_l i out )) ,
+  ((( &( "found" ) )) # Ptr  |->_)
+  **  ((( &( "ch" ) )) # Int  |-> (Znth i (c_string (str_l)) 0))
+  **  ((( &( "num" ) )) # Ptr  |-> num_pre)
+  **  ((( &( "key" ) )) # Ptr  |-> key)
+  **  ((( &( "n" ) )) # Int  |-> n)
+  **  ((( &( "i" ) )) # Int  |-> i)
+  **  ((( &( "out" ) )) # Int  |-> out)
+  **  (store_string num_pre str_l )
+  **  (store_string key key_payload_78 )
+  **  (GlobalStrings_missing LitMap all_key_literals_78 )
+|--
+  “ ((string_length (key_payload_78)) < INT_MAX) ” 
+  &&  “ ((Znth i (c_string (str_l)) 0) <= 127) ” 
+  &&  “ (0 <= (Znth i (c_string (str_l)) 0)) ” 
+  &&  “ (valid_string key_payload_78 ) ”
+) \/
+(
+forall (num_pre: Z) (str_l: (@list Z)) (out: Z) (i: Z) (n: Z) (key: Z) (PreH1 : (out <= INT_MAX)) (PreH2 : (i <= INT_MAX)) (PreH3 : (n <= INT_MAX)) (PreH4 : ((Znth i (c_string (str_l)) 0) <= INT_MAX)) (PreH5 : (out >= INT_MIN)) (PreH6 : (i >= INT_MIN)) (PreH7 : (n >= INT_MIN)) (PreH8 : ((Znth i (c_string (str_l)) 0) >= INT_MIN)) (PreH9 : (0 <= ((string_length (key_payload_78)) + 1 ))) (PreH10 : (0 <= ((string_length (str_l)) + 1 ))) (PreH11 : (i < n)) (PreH12 : (key = (key_ptr_78 (LitMap)))) (PreH13 : (n = (string_length (str_l)))) (PreH14 : (0 <= i)) (PreH15 : (i <= n)) (PreH16 : (0 <= out)) (PreH17 : (out <= i)) (PreH18 : (valid_string str_l )) (PreH19 : (all_ascii str_l )) (PreH20 : (problem_78_pre_z str_l )) (PreH21 : (hex_count_safe_78 str_l )) (PreH22 : (key_payload_safe_78 )) (PreH23 : ((string_length (str_l)) < INT_MAX)) (PreH24 : (hex_count_state_78 str_l i out )) ,
+  (CharArray.full key ((string_length (key_payload_78)) + 1 ) (c_string (key_payload_78)) )
+  **  (CharArray.full num_pre ((string_length (str_l)) + 1 ) (c_string (str_l)) )
+  **  ((( &( "found" ) )) # Ptr  |->_)
+  **  ((( &( "ch" ) )) # Int  |-> (Znth i (c_string (str_l)) 0))
+  **  ((( &( "num" ) )) # Ptr  |-> num_pre)
+  **  ((( &( "key" ) )) # Ptr  |-> key)
+  **  ((( &( "n" ) )) # Int  |-> n)
+  **  ((( &( "i" ) )) # Int  |-> i)
+  **  ((( &( "out" ) )) # Int  |-> out)
+  **  (GlobalStrings_missing LitMap all_key_literals_78 )
+|--
+  “ (valid_string key_payload_78 ) ” 
+  &&  “ (0 <= (Znth i (c_string (str_l)) 0)) ” 
+  &&  “ ((Znth i (c_string (str_l)) 0) <= 127) ” 
+  &&  “ ((string_length (key_payload_78)) < INT_MAX) ”
+).
+
+Definition hex_key_partial_solve_wit_2_pure_split_goal_1 := 
+forall (num_pre: Z) (str_l: (@list Z)) (out: Z) (i: Z) (n: Z) (key: Z) (PreH1 : (out <= INT_MAX)) (PreH2 : (i <= INT_MAX)) (PreH3 : (n <= INT_MAX)) (PreH4 : ((Znth i (c_string (str_l)) 0) <= INT_MAX)) (PreH5 : (out >= INT_MIN)) (PreH6 : (i >= INT_MIN)) (PreH7 : (n >= INT_MIN)) (PreH8 : ((Znth i (c_string (str_l)) 0) >= INT_MIN)) (PreH9 : (0 <= ((string_length (key_payload_78)) + 1 ))) (PreH10 : (0 <= ((string_length (str_l)) + 1 ))) (PreH11 : (i < n)) (PreH12 : (key = (key_ptr_78 (LitMap)))) (PreH13 : (n = (string_length (str_l)))) (PreH14 : (0 <= i)) (PreH15 : (i <= n)) (PreH16 : (0 <= out)) (PreH17 : (out <= i)) (PreH18 : (valid_string str_l )) (PreH19 : (all_ascii str_l )) (PreH20 : (problem_78_pre_z str_l )) (PreH21 : (hex_count_safe_78 str_l )) (PreH22 : (key_payload_safe_78 )) (PreH23 : ((string_length (str_l)) < INT_MAX)) (PreH24 : (hex_count_state_78 str_l i out )) ,
+  (CharArray.full key ((string_length (key_payload_78)) + 1 ) (c_string (key_payload_78)) )
+  **  (CharArray.full num_pre ((string_length (str_l)) + 1 ) (c_string (str_l)) )
+  **  ((( &( "found" ) )) # Ptr  |->_)
+  **  ((( &( "ch" ) )) # Int  |-> (Znth i (c_string (str_l)) 0))
+  **  ((( &( "num" ) )) # Ptr  |-> num_pre)
+  **  ((( &( "key" ) )) # Ptr  |-> key)
+  **  ((( &( "n" ) )) # Int  |-> n)
+  **  ((( &( "i" ) )) # Int  |-> i)
+  **  ((( &( "out" ) )) # Int  |-> out)
+  **  (GlobalStrings_missing LitMap all_key_literals_78 )
+|--
+  “ (valid_string key_payload_78 ) ”
+.
+
+Definition hex_key_partial_solve_wit_2_pure_split_goal_2 := 
+forall (num_pre: Z) (str_l: (@list Z)) (out: Z) (i: Z) (n: Z) (key: Z) (PreH1 : (out <= INT_MAX)) (PreH2 : (i <= INT_MAX)) (PreH3 : (n <= INT_MAX)) (PreH4 : ((Znth i (c_string (str_l)) 0) <= INT_MAX)) (PreH5 : (out >= INT_MIN)) (PreH6 : (i >= INT_MIN)) (PreH7 : (n >= INT_MIN)) (PreH8 : ((Znth i (c_string (str_l)) 0) >= INT_MIN)) (PreH9 : (0 <= ((string_length (key_payload_78)) + 1 ))) (PreH10 : (0 <= ((string_length (str_l)) + 1 ))) (PreH11 : (i < n)) (PreH12 : (key = (key_ptr_78 (LitMap)))) (PreH13 : (n = (string_length (str_l)))) (PreH14 : (0 <= i)) (PreH15 : (i <= n)) (PreH16 : (0 <= out)) (PreH17 : (out <= i)) (PreH18 : (valid_string str_l )) (PreH19 : (all_ascii str_l )) (PreH20 : (problem_78_pre_z str_l )) (PreH21 : (hex_count_safe_78 str_l )) (PreH22 : (key_payload_safe_78 )) (PreH23 : ((string_length (str_l)) < INT_MAX)) (PreH24 : (hex_count_state_78 str_l i out )) ,
+  (CharArray.full key ((string_length (key_payload_78)) + 1 ) (c_string (key_payload_78)) )
+  **  (CharArray.full num_pre ((string_length (str_l)) + 1 ) (c_string (str_l)) )
+  **  ((( &( "found" ) )) # Ptr  |->_)
+  **  ((( &( "ch" ) )) # Int  |-> (Znth i (c_string (str_l)) 0))
+  **  ((( &( "num" ) )) # Ptr  |-> num_pre)
+  **  ((( &( "key" ) )) # Ptr  |-> key)
+  **  ((( &( "n" ) )) # Int  |-> n)
+  **  ((( &( "i" ) )) # Int  |-> i)
+  **  ((( &( "out" ) )) # Int  |-> out)
+  **  (GlobalStrings_missing LitMap all_key_literals_78 )
+|--
+  “ (0 <= (Znth i (c_string (str_l)) 0)) ”
+.
+
+Definition hex_key_partial_solve_wit_2_pure_split_goal_3 := 
+forall (num_pre: Z) (str_l: (@list Z)) (out: Z) (i: Z) (n: Z) (key: Z) (PreH1 : (out <= INT_MAX)) (PreH2 : (i <= INT_MAX)) (PreH3 : (n <= INT_MAX)) (PreH4 : ((Znth i (c_string (str_l)) 0) <= INT_MAX)) (PreH5 : (out >= INT_MIN)) (PreH6 : (i >= INT_MIN)) (PreH7 : (n >= INT_MIN)) (PreH8 : ((Znth i (c_string (str_l)) 0) >= INT_MIN)) (PreH9 : (0 <= ((string_length (key_payload_78)) + 1 ))) (PreH10 : (0 <= ((string_length (str_l)) + 1 ))) (PreH11 : (i < n)) (PreH12 : (key = (key_ptr_78 (LitMap)))) (PreH13 : (n = (string_length (str_l)))) (PreH14 : (0 <= i)) (PreH15 : (i <= n)) (PreH16 : (0 <= out)) (PreH17 : (out <= i)) (PreH18 : (valid_string str_l )) (PreH19 : (all_ascii str_l )) (PreH20 : (problem_78_pre_z str_l )) (PreH21 : (hex_count_safe_78 str_l )) (PreH22 : (key_payload_safe_78 )) (PreH23 : ((string_length (str_l)) < INT_MAX)) (PreH24 : (hex_count_state_78 str_l i out )) ,
+  (CharArray.full key ((string_length (key_payload_78)) + 1 ) (c_string (key_payload_78)) )
+  **  (CharArray.full num_pre ((string_length (str_l)) + 1 ) (c_string (str_l)) )
+  **  ((( &( "found" ) )) # Ptr  |->_)
+  **  ((( &( "ch" ) )) # Int  |-> (Znth i (c_string (str_l)) 0))
+  **  ((( &( "num" ) )) # Ptr  |-> num_pre)
+  **  ((( &( "key" ) )) # Ptr  |-> key)
+  **  ((( &( "n" ) )) # Int  |-> n)
+  **  ((( &( "i" ) )) # Int  |-> i)
+  **  ((( &( "out" ) )) # Int  |-> out)
+  **  (GlobalStrings_missing LitMap all_key_literals_78 )
+|--
+  “ ((Znth i (c_string (str_l)) 0) <= 127) ”
+.
+
+Definition hex_key_partial_solve_wit_2_pure_split_goal_4 := 
+forall (num_pre: Z) (str_l: (@list Z)) (out: Z) (i: Z) (n: Z) (key: Z) (PreH1 : (out <= INT_MAX)) (PreH2 : (i <= INT_MAX)) (PreH3 : (n <= INT_MAX)) (PreH4 : ((Znth i (c_string (str_l)) 0) <= INT_MAX)) (PreH5 : (out >= INT_MIN)) (PreH6 : (i >= INT_MIN)) (PreH7 : (n >= INT_MIN)) (PreH8 : ((Znth i (c_string (str_l)) 0) >= INT_MIN)) (PreH9 : (0 <= ((string_length (key_payload_78)) + 1 ))) (PreH10 : (0 <= ((string_length (str_l)) + 1 ))) (PreH11 : (i < n)) (PreH12 : (key = (key_ptr_78 (LitMap)))) (PreH13 : (n = (string_length (str_l)))) (PreH14 : (0 <= i)) (PreH15 : (i <= n)) (PreH16 : (0 <= out)) (PreH17 : (out <= i)) (PreH18 : (valid_string str_l )) (PreH19 : (all_ascii str_l )) (PreH20 : (problem_78_pre_z str_l )) (PreH21 : (hex_count_safe_78 str_l )) (PreH22 : (key_payload_safe_78 )) (PreH23 : ((string_length (str_l)) < INT_MAX)) (PreH24 : (hex_count_state_78 str_l i out )) ,
+  (CharArray.full key ((string_length (key_payload_78)) + 1 ) (c_string (key_payload_78)) )
+  **  (CharArray.full num_pre ((string_length (str_l)) + 1 ) (c_string (str_l)) )
+  **  ((( &( "found" ) )) # Ptr  |->_)
+  **  ((( &( "ch" ) )) # Int  |-> (Znth i (c_string (str_l)) 0))
+  **  ((( &( "num" ) )) # Ptr  |-> num_pre)
+  **  ((( &( "key" ) )) # Ptr  |-> key)
+  **  ((( &( "n" ) )) # Int  |-> n)
+  **  ((( &( "i" ) )) # Int  |-> i)
+  **  ((( &( "out" ) )) # Int  |-> out)
+  **  (GlobalStrings_missing LitMap all_key_literals_78 )
+|--
+  “ ((string_length (key_payload_78)) < INT_MAX) ”
+.
+
+Definition hex_key_partial_solve_wit_2_aux := 
+forall (num_pre: Z) (str_l: (@list Z)) (out: Z) (i: Z) (n: Z) (key: Z) (PreH1 : (i < n)) (PreH2 : (key = (key_ptr_78 (LitMap)))) (PreH3 : (n = (string_length (str_l)))) (PreH4 : (0 <= i)) (PreH5 : (i <= n)) (PreH6 : (0 <= out)) (PreH7 : (out <= i)) (PreH8 : (valid_string str_l )) (PreH9 : (all_ascii str_l )) (PreH10 : (problem_78_pre_z str_l )) (PreH11 : (hex_count_safe_78 str_l )) (PreH12 : (key_payload_safe_78 )) (PreH13 : ((string_length (str_l)) < INT_MAX)) (PreH14 : (hex_count_state_78 str_l i out )) ,
+  (store_string num_pre str_l )
+  **  (store_string key key_payload_78 )
+  **  (GlobalStrings_missing LitMap all_key_literals_78 )
+|--
+  “ ((string_length (key_payload_78)) < INT_MAX) ” 
+  &&  “ ((Znth i (c_string (str_l)) 0) <= 127) ” 
+  &&  “ (0 <= (Znth i (c_string (str_l)) 0)) ” 
+  &&  “ (valid_string key_payload_78 ) ” 
+  &&  “ (0 <= ((string_length (key_payload_78)) + 1 )) ” 
+  &&  “ (0 <= ((string_length (str_l)) + 1 )) ” 
+  &&  “ (i < n) ” 
+  &&  “ (key = (key_ptr_78 (LitMap))) ” 
+  &&  “ (n = (string_length (str_l))) ” 
+  &&  “ (0 <= i) ” 
+  &&  “ (i <= n) ” 
+  &&  “ (0 <= out) ” 
+  &&  “ (out <= i) ” 
+  &&  “ (valid_string str_l ) ” 
+  &&  “ (all_ascii str_l ) ” 
+  &&  “ (problem_78_pre_z str_l ) ” 
+  &&  “ (hex_count_safe_78 str_l ) ” 
+  &&  “ (key_payload_safe_78 ) ” 
+  &&  “ ((string_length (str_l)) < INT_MAX) ” 
+  &&  “ (hex_count_state_78 str_l i out ) ”
+  &&  (store_string key key_payload_78 )
+  **  (CharArray.full num_pre ((string_length (str_l)) + 1 ) (c_string (str_l)) )
+  **  (GlobalStrings_missing LitMap all_key_literals_78 )
+.
+
+Definition hex_key_partial_solve_wit_2 := hex_key_partial_solve_wit_2_pure -> hex_key_partial_solve_wit_2_aux.
+
+Module Type VC_Correct.
+
+Include char_array_Strategy_Correct.
+Include string_Strategy_Correct.
+
+Axiom proof_of_hex_key_safety_wit_1 : hex_key_safety_wit_1.
+Axiom proof_of_hex_key_safety_wit_2 : hex_key_safety_wit_2.
+Axiom proof_of_hex_key_safety_wit_3 : hex_key_safety_wit_3.
+Axiom proof_of_hex_key_safety_wit_4 : hex_key_safety_wit_4.
+Axiom proof_of_hex_key_safety_wit_5 : hex_key_safety_wit_5.
+Axiom proof_of_hex_key_safety_wit_6 : hex_key_safety_wit_6.
+Axiom proof_of_hex_key_safety_wit_7 : hex_key_safety_wit_7.
+Axiom proof_of_hex_key_safety_wit_8 : hex_key_safety_wit_8.
+Axiom proof_of_hex_key_entail_wit_1 : hex_key_entail_wit_1.
+Axiom proof_of_hex_key_entail_wit_2 : hex_key_entail_wit_2.
+Axiom proof_of_hex_key_entail_wit_3 : hex_key_entail_wit_3.
+Axiom proof_of_hex_key_entail_wit_4 : hex_key_entail_wit_4.
+Axiom proof_of_hex_key_entail_wit_5_1 : hex_key_entail_wit_5_1.
+Axiom proof_of_hex_key_entail_wit_5_2 : hex_key_entail_wit_5_2.
+Axiom proof_of_hex_key_entail_wit_6 : hex_key_entail_wit_6.
+Axiom proof_of_hex_key_return_wit_1 : hex_key_return_wit_1.
+Axiom proof_of_hex_key_partial_solve_wit_1_pure : hex_key_partial_solve_wit_1_pure.
+Axiom proof_of_hex_key_partial_solve_wit_1 : hex_key_partial_solve_wit_1.
+Axiom proof_of_hex_key_partial_solve_wit_2_pure : hex_key_partial_solve_wit_2_pure.
+Axiom proof_of_hex_key_partial_solve_wit_2 : hex_key_partial_solve_wit_2.
+
+End VC_Correct.
