QCP_examples/humaneval/spec_logic_rewrite_c_files/C_78_proof_manual.v
@@ -1,0 +1,134 @@
+Require Import Coq.ZArith.ZArith.
+Require Import Coq.Bool.Bool.
+Require Import Coq.Strings.String.
+Require Import Coq.Strings.Ascii.
+Require Import Coq.Lists.List.
+Require Import Coq.Classes.RelationClasses.
+Require Import Coq.Classes.Morphisms.
+Require Import Coq.micromega.Psatz.
+Require Import Coq.Sorting.Permutation.
+From AUXLib Require Import int_auto Axioms Feq Idents ListLib VMap.
+Require Import SetsClass.SetsClass. Import SetsNotation.
+From SimpleC.SL Require Import Mem SeparationLogic.
+From SimpleC.EE Require Import C_78_goal.
+From SimpleC.EE Require Import C_78_proof_auto.
+Require Import Logic.LogicGenerator.demo932.Interface.
+Local Open Scope Z_scope.
+Local Open Scope sets.
+Local Open Scope string_scope.
+Local Open Scope list.
+Import naive_C_Rules.
+Require Import SimpleC.StdLib.string_lib.
+Require Import coins_78.
+Local Open Scope sac.
+
+Ltac c78_char_bounds :=
+  match goal with
+  | |- 0 <= Znth ?k (c_string ?s) 0 =>
+      pose proof (all_ascii_c_string_inside_78 s k ltac:(assumption) ltac:(lia));
+      lia
+  | |- Znth ?k (c_string ?s) 0 <= 127 =>
+      pose proof (all_ascii_c_string_inside_78 s k ltac:(assumption) ltac:(lia));
+      lia
+  end.
+
+Ltac c78_finish :=
+  entailer!; eauto; try c78_char_bounds; try lia.
+
+Lemma proof_of_hex_key_entail_wit_1 : hex_key_entail_wit_1.
+Proof.
+  right.
+  pre_process_default.
+  pose proof key_payload_safe_proof_78.
+  sep_apply_l_atomic (GlobalStrings_split LitMap key_literal_78).
+  sep_apply_l_atomic (key_lit_to_store_78 LitMap).
+  unfold all_key_literals_78, key_ptr_78, key_literal_78,
+    key_payload_78, string_lib.store_string.
+  simpl.
+  replace (LitMap "2357BD" + 0) with (LitMap "2357BD") by lia.
+  entailer!.
+Qed. 
+
+Lemma proof_of_hex_key_entail_wit_2 : hex_key_entail_wit_2.
+Proof.
+  right.
+  pre_process_default.
+  entailer!.
+  - subst retval. apply string_length_nonneg.
+  - apply hex_count_initial_78.
+Qed. 
+
+Lemma proof_of_hex_key_entail_wit_3 : hex_key_entail_wit_3.
+Proof.
+  right.
+  pre_process_default.
+  assert (Hi : 0 <= i < string_length str_l) by (subst n; lia).
+  assert (Hrange : 0 <= Znth i (c_string str_l) 0 <= 127) by
+    (apply all_ascii_c_string_inside_78; [exact PreH13 | exact Hi]).
+  assert (Hnz : Znth i (c_string str_l) 0 <> 0) by
+    (apply c_string_nonzero_inside_78; [exact PreH12 | exact Hi]).
+  assert (Hprime : prime_hex_code_78 (Znth i (c_string str_l) 0)) by
+    (eapply strchr_result_key_hit_prime_78; eauto).
+  assert (Hstep : hex_hit_step_78 str_l i (out + 1)).
+  {
+    eapply hex_hit_step_intro_78; eauto.
+    replace ((out + 1) - 1) with out by lia.
+    exact PreH18.
+  }
+  assert (Hstate : hex_count_state_78 str_l (i + 1) (out + 1)) by
+    (destruct Hstep as [_ [_ Hstate]]; exact Hstate).
+  entailer!; eauto; lia.
+Qed. 
+
+Lemma proof_of_hex_key_entail_wit_4 : hex_key_entail_wit_4.
+Proof.
+  right.
+  pre_process_default.
+  assert (Hi : 0 <= i < string_length str_l) by (subst n; lia).
+  assert (Hrange : 0 <= Znth i (c_string str_l) 0 <= 127) by
+    (apply all_ascii_c_string_inside_78; [exact PreH13 | exact Hi]).
+  assert (Hmiss : ~ prime_hex_code_78 (Znth i (c_string str_l) 0)) by
+    (subst retval; eapply strchr_result_key_miss_not_prime_78; eauto).
+  assert (Hstep : hex_miss_step_78 str_l i out) by
+    (eapply hex_miss_step_intro_78; eauto).
+  assert (Hstate : hex_count_state_78 str_l (i + 1) out) by
+    (destruct Hstep as [_ [_ Hstate]]; exact Hstate).
+  entailer!; eauto; lia.
+Qed. 
+
+Lemma proof_of_hex_key_entail_wit_6 : hex_key_entail_wit_6.
+Proof.
+  right.
+  pre_process_default.
+  assert (Hi_eq : i = n) by lia.
+  assert (Hstate_len : hex_count_state_78 str_l (string_length str_l) out).
+  {
+    replace (string_length str_l) with i by lia.
+    exact PreH16.
+  }
+  assert (Hfinal : hex_final_78 str_l out) by
+    (eapply hex_final_from_safe_78; [exact PreH13 | exact Hstate_len]).
+  pose proof Hfinal as Hfinal_keep.
+  destruct Hfinal as [Hstate_final Hspec].
+  assert (Hstate_n : hex_count_state_78 str_l n out) by
+    (subst n; exact Hstate_final).
+  entailer!; eauto.
+Qed. 
+
+Lemma proof_of_hex_key_return_wit_1 : hex_key_return_wit_1.
+Proof.
+  left.
+  pre_process.
+  subst key.
+  entailer!.
+Qed. 
+
+Lemma proof_of_hex_key_partial_solve_wit_2_pure : hex_key_partial_solve_wit_2_pure.
+Proof.
+  right.
+  pre_process_default.
+  destruct PreH22 as [Hvalid_key [Hascii_key Hlen_key]].
+  assert (Hi : 0 <= i < string_length str_l) by (subst n; lia).
+  pose proof (all_ascii_c_string_inside_78 str_l i PreH19 Hi) as Hchar.
+  entailer!; lia.
+Qed. 
