QCP_examples/humaneval/spec_logic_rewrite_c_files/coins_78.v
@@ -1,0 +1,497 @@
+Load "../spec/78".
+
+Require Import Coq.ZArith.ZArith.
+Require Import Coq.Bool.Bool.
+Require Import Coq.Lists.List.
+Require Import Coq.Strings.String.
+Require Import Coq.Strings.Ascii.
+Require Import Lia.
+From AUXLib Require Import ListLib.
+From SimpleC.SL Require Import IntLib Mem SeparationLogic.
+Require Import SimpleC.StdLib.string_lib.
+
+Import ListNotations.
+
+Local Open Scope Z_scope.
+Local Open Scope string_scope.
+Local Open Scope list_scope.
+Import naive_C_Rules.
+Local Open Scope sac.
+
+Parameter LitMap : string -> addr.
+
+Definition ascii_of_z_78 (z : Z) : ascii :=
+  ascii_of_nat (Z.to_nat z).
+
+Fixpoint string_of_list_z_78 (l : list Z) : string :=
+  match l with
+  | [] => EmptyString
+  | c :: rest => String (ascii_of_z_78 c) (string_of_list_z_78 rest)
+  end.
+
+Definition problem_78_pre_z (s : list Z) : Prop :=
+  problem_78_pre (string_of_list_z_78 s).
+
+Definition problem_78_spec_z (s : list Z) (output : Z) : Prop :=
+  problem_78_spec (string_of_list_z_78 s) (Z.to_nat output).
+
+Definition key_literal_78 : string := "2357BD"%string.
+
+Definition all_key_literals_78 : list string :=
+  [key_literal_78].
+
+Definition key_payload_78 : list Z :=
+  [50; 51; 53; 55; 66; 68].
+
+Definition key_ptr_78 (LM : string -> Z) : Z :=
+  LM key_literal_78.
+
+Definition key_payload_safe_78 : Prop :=
+  string_lib.valid_string key_payload_78 /\
+  all_ascii key_payload_78 /\
+  string_length key_payload_78 < INT_MAX.
+
+Definition key_literal_heap_78 (LM : string -> Z) : Assertion :=
+  string_lib.store_string (key_ptr_78 LM) key_payload_78 **
+  GlobalStrings_missing LM all_key_literals_78.
+
+Definition is_prime_hex_z_78 (c : Z) : bool :=
+  is_prime_hex_digit (ascii_of_z_78 c).
+
+Definition prime_hex_code_78 (c : Z) : Prop :=
+  is_prime_hex_z_78 c = true.
+
+Fixpoint count_prime_hex_list_z_78 (l : list Z) : Z :=
+  match l with
+  | [] => 0
+  | c :: rest =>
+      (if is_prime_hex_z_78 c then 1 else 0) +
+      count_prime_hex_list_z_78 rest
+  end.
+
+Definition hex_count_upto_78 (i : Z) (s : list Z) : Z :=
+  count_prime_hex_list_z_78 (firstn (Z.to_nat i) (c_string s)).
+
+Definition hex_count_state_78 (s : list Z) (i count : Z) : Prop :=
+  0 <= i <= string_length s /\
+  count = hex_count_upto_78 i s /\
+  0 <= count <= i.
+
+Definition hex_hit_step_78 (s : list Z) (i count : Z) : Prop :=
+  0 <= i < string_length s /\
+  prime_hex_code_78 (Znth i (c_string s) 0) /\
+  hex_count_state_78 s (i + 1) count.
+
+Definition hex_miss_step_78 (s : list Z) (i count : Z) : Prop :=
+  0 <= i < string_length s /\
+  ~ prime_hex_code_78 (Znth i (c_string s) 0) /\
+  hex_count_state_78 s (i + 1) count.
+
+Definition hex_final_78 (s : list Z) (count : Z) : Prop :=
+  hex_count_state_78 s (string_length s) count /\
+  problem_78_spec_z s count.
+
+Definition hex_count_safe_78 (s : list Z) : Prop :=
+  hex_count_state_78 s 0 0 /\
+  (forall i count,
+      hex_count_state_78 s i (count - 1) ->
+      0 <= i < string_length s ->
+      prime_hex_code_78 (Znth i (c_string s) 0) ->
+      hex_hit_step_78 s i count) /\
+  (forall i count,
+      hex_count_state_78 s i count ->
+      0 <= i < string_length s ->
+      ~ prime_hex_code_78 (Znth i (c_string s) 0) ->
+      hex_miss_step_78 s i count) /\
+  (forall count,
+      hex_count_state_78 s (string_length s) count ->
+      hex_final_78 s count).
+
+Lemma list_ascii_of_string_of_list_z_78 : forall l,
+  list_ascii_of_string (string_of_list_z_78 l) =
+  map ascii_of_z_78 l.
+Proof.
+  induction l as [| c rest IH]; simpl; congruence.
+Qed.
+
+Lemma count_prime_hex_list_z_nonneg_78 : forall l,
+  0 <= count_prime_hex_list_z_78 l.
+Proof.
+  induction l as [| c rest IH]; simpl.
+  - lia.
+  - destruct (is_prime_hex_z_78 c); lia.
+Qed.
+
+Lemma firstn_succ_snoc_78 : forall {A : Type} n (l : list A) d,
+  (n < List.length l)%nat ->
+  firstn (S n) l = firstn n l ++ [nth n l d].
+Proof.
+  induction n.
+  - intros l d Hn. destruct l; simpl in *; try lia. reflexivity.
+  - intros l d Hn. destruct l; simpl in *; try lia.
+    rewrite (IHn l d) by lia. reflexivity.
+Qed.
+
+Lemma firstn_succ_Znth_78 : forall (l : list Z) i,
+  0 <= i < Zlength l ->
+  firstn (Z.to_nat (i + 1)) l =
+  firstn (Z.to_nat i) l ++ [Znth i l 0].
+Proof.
+  intros l i H.
+  replace (Z.to_nat (i + 1)) with (S (Z.to_nat i)) by lia.
+  rewrite firstn_succ_snoc_78 with (d := 0)
+    by (rewrite Zlength_correct in H; lia).
+  reflexivity.
+Qed.
+
+Lemma count_prime_hex_list_z_app_78 : forall l1 l2,
+  count_prime_hex_list_z_78 (l1 ++ l2) =
+  count_prime_hex_list_z_78 l1 + count_prime_hex_list_z_78 l2.
+Proof.
+  induction l1 as [| c rest IH]; intros l2; simpl.
+  - lia.
+  - rewrite IH. lia.
+Qed.
+
+Lemma hex_count_upto_step_hit_78 : forall s i,
+  0 <= i < string_length s ->
+  prime_hex_code_78 (Znth i (c_string s) 0) ->
+  hex_count_upto_78 (i + 1) s =
+  hex_count_upto_78 i s + 1.
+Proof.
+  intros s i Hi Hprime.
+  unfold hex_count_upto_78.
+  rewrite firstn_succ_Znth_78
+    by (unfold string_length, c_string in *; rewrite Zlength_app, Zlength_cons, Zlength_nil; lia).
+  rewrite count_prime_hex_list_z_app_78.
+  simpl.
+  rewrite Hprime.
+  lia.
+Qed.
+
+Lemma hex_count_upto_step_miss_78 : forall s i,
+  0 <= i < string_length s ->
+  ~ prime_hex_code_78 (Znth i (c_string s) 0) ->
+  hex_count_upto_78 (i + 1) s =
+  hex_count_upto_78 i s.
+Proof.
+  intros s i Hi Hmiss.
+  unfold hex_count_upto_78.
+  rewrite firstn_succ_Znth_78
+    by (unfold string_length, c_string in *; rewrite Zlength_app, Zlength_cons, Zlength_nil; lia).
+  rewrite count_prime_hex_list_z_app_78.
+  simpl.
+  destruct (is_prime_hex_z_78 (Znth i (c_string s) 0)) eqn:Hprime; [| lia].
+  exfalso.
+  apply Hmiss.
+  exact Hprime.
+Qed.
+
+Lemma count_prime_hex_list_z_length_filter_78 : forall l,
+  Z.to_nat (count_prime_hex_list_z_78 l) =
+  List.length (filter is_prime_hex_digit (map ascii_of_z_78 l)).
+Proof.
+  induction l as [| c rest IH]; simpl.
+  - reflexivity.
+  - destruct (is_prime_hex_z_78 c) eqn:Hc; unfold is_prime_hex_z_78 in Hc; rewrite Hc; simpl.
+    + change (Z.to_nat (1 + count_prime_hex_list_z_78 rest) =
+              S (List.length (filter is_prime_hex_digit (map ascii_of_z_78 rest)))).
+      rewrite Z2Nat.inj_add by (pose proof (count_prime_hex_list_z_nonneg_78 rest); lia).
+      rewrite IH. reflexivity.
+    + exact IH.
+Qed.
+
+Lemma filter_prime_hex_digits_78 : forall s,
+  prime_hex_digits
+    s
+    (filter is_prime_hex_digit (list_ascii_of_string s)).
+Proof.
+  intros s.
+  unfold prime_hex_digits, prime_hex_digit.
+  split.
+  - intros c Hin.
+    apply filter_In in Hin.
+    tauto.
+  - intros c Hin Hprime.
+    apply filter_In.
+    tauto.
+Qed.
+
+Lemma problem_78_spec_z_intro : forall s output,
+  output = count_prime_hex_list_z_78 s ->
+  problem_78_spec_z s output.
+Proof.
+  intros s output Hout.
+  unfold problem_78_spec_z, problem_78_spec.
+  exists (filter is_prime_hex_digit (list_ascii_of_string (string_of_list_z_78 s))).
+  split.
+  - apply filter_prime_hex_digits_78.
+  - rewrite Hout.
+    rewrite list_ascii_of_string_of_list_z_78.
+    rewrite count_prime_hex_list_z_length_filter_78.
+    reflexivity.
+Qed.
+
+Lemma hex_count_initial_78 : forall s,
+  hex_count_state_78 s 0 0.
+Proof.
+  intros s.
+  unfold hex_count_state_78, hex_count_upto_78.
+  split; [unfold string_length; rewrite Zlength_correct; lia |].
+  split; [reflexivity | lia].
+Qed.
+
+Lemma hex_hit_step_intro_78 : forall s i count,
+  hex_count_state_78 s i (count - 1) ->
+  0 <= i < string_length s ->
+  prime_hex_code_78 (Znth i (c_string s) 0) ->
+  hex_hit_step_78 s i count.
+Proof.
+  intros s i count Hstate Hi Hprime.
+  unfold hex_hit_step_78.
+  split; [exact Hi | split; [exact Hprime |]].
+  unfold hex_count_state_78 in *.
+  destruct Hstate as [_ [Hcount Hbound]].
+  split; [lia | split].
+  - rewrite hex_count_upto_step_hit_78 by assumption. lia.
+  - lia.
+Qed.
+
+Lemma hex_miss_step_intro_78 : forall s i count,
+  hex_count_state_78 s i count ->
+  0 <= i < string_length s ->
+  ~ prime_hex_code_78 (Znth i (c_string s) 0) ->
+  hex_miss_step_78 s i count.
+Proof.
+  intros s i count Hstate Hi Hmiss.
+  unfold hex_miss_step_78.
+  split; [exact Hi | split; [exact Hmiss |]].
+  unfold hex_count_state_78 in *.
+  destruct Hstate as [_ [Hcount Hbound]].
+  split; [lia | split].
+  - rewrite hex_count_upto_step_miss_78 by assumption. lia.
+  - lia.
+Qed.
+
+Lemma hex_final_intro_78 : forall s count,
+  hex_count_state_78 s (string_length s) count ->
+  hex_final_78 s count.
+Proof.
+  intros s count Hstate.
+  unfold hex_final_78.
+  split; [exact Hstate |].
+  unfold hex_count_state_78 in Hstate.
+  destruct Hstate as [_ [Hcount _]].
+  unfold hex_count_upto_78 in Hcount.
+  unfold c_string in Hcount.
+  replace (Z.to_nat (string_length s)) with (List.length s) in Hcount
+    by (unfold string_length; rewrite Zlength_correct; lia).
+  rewrite firstn_app in Hcount.
+  rewrite firstn_all in Hcount.
+  replace (List.length s - List.length s)%nat with 0%nat in Hcount by lia.
+  simpl in Hcount.
+  rewrite List.app_nil_r in Hcount.
+  apply problem_78_spec_z_intro.
+  exact Hcount.
+Qed.
+
+Lemma hex_count_safe_intro_78 : forall s,
+  hex_count_safe_78 s.
+Proof.
+  intro s.
+  unfold hex_count_safe_78.
+  split.
+  - apply hex_count_initial_78.
+  - split.
+    + intros i count Hstate Hi Hprime.
+      apply hex_hit_step_intro_78; assumption.
+    + split.
+      * intros i count Hstate Hi Hmiss.
+        apply hex_miss_step_intro_78; assumption.
+      * intros count Hstate.
+        apply hex_final_intro_78; assumption.
+Qed.
+
+Lemma all_ascii_c_string_inside_78 : forall s i,
+  all_ascii s ->
+  0 <= i < string_length s ->
+  0 <= Znth i (c_string s) 0 <= 127.
+Proof.
+  intros s i Hascii Hi.
+  rewrite c_string_Znth_inside by exact Hi.
+  apply Hascii.
+  unfold string_length in Hi.
+  exact Hi.
+Qed.
+
+Lemma c_string_nonzero_inside_78 : forall s i,
+  string_lib.valid_string s ->
+  0 <= i < string_length s ->
+  Znth i (c_string s) 0 <> 0.
+Proof.
+  intros s i Hvalid Hi.
+  rewrite c_string_Znth_inside by exact Hi.
+  destruct Hvalid as [_ Hno].
+  apply Hno.
+  unfold string_length in Hi.
+  exact Hi.
+Qed.
+
+Lemma key_lit_to_store_78 : forall LM,
+  store_stringLit (LM key_literal_78) key_literal_78 |--
+  string_lib.store_string (key_ptr_78 LM) key_payload_78.
+Proof.
+  intros.
+  unfold store_stringLit, string_lib.store_string.
+  unfold key_ptr_78, key_payload_78, key_literal_78.
+  simpl.
+  entailer!.
+Qed.
+
+Lemma key_payload_safe_proof_78 : key_payload_safe_78.
+Proof.
+  unfold key_payload_safe_78, string_lib.valid_string, string_lib.all_ascii,
+    string_lib.no_inner_nul, all_ascii, no_inner_nul, string_length,
+    key_payload_78, key_literal_78.
+  assert (Hascii :
+    forall i : Z,
+      0 <= i < Zlength [50; 51; 53; 55; 66; 68] ->
+      0 <= Znth i [50; 51; 53; 55; 66; 68] 0 <= 127).
+  {
+    intros i Hi.
+    change (Zlength [50; 51; 53; 55; 66; 68]) with 6 in Hi.
+    assert (i = 0 \/ i = 1 \/ i = 2 \/ i = 3 \/ i = 4 \/ i = 5) by lia.
+    destruct H as [-> | [-> | [-> | [-> | [-> | ->]]]]];
+    try change (Znth 0 [50; 51; 53; 55; 66; 68] 0) with 50;
+    try change (Znth 1 [50; 51; 53; 55; 66; 68] 0) with 51;
+    try change (Znth 2 [50; 51; 53; 55; 66; 68] 0) with 53;
+    try change (Znth 3 [50; 51; 53; 55; 66; 68] 0) with 55;
+    try change (Znth 4 [50; 51; 53; 55; 66; 68] 0) with 66;
+    try change (Znth 5 [50; 51; 53; 55; 66; 68] 0) with 68;
+    lia.
+  }
+  assert (Hnonzero :
+    forall i : Z,
+      0 <= i < Zlength [50; 51; 53; 55; 66; 68] ->
+      Znth i [50; 51; 53; 55; 66; 68] 0 <> 0).
+  {
+    intros i Hi.
+    change (Zlength [50; 51; 53; 55; 66; 68]) with 6 in Hi.
+    assert (i = 0 \/ i = 1 \/ i = 2 \/ i = 3 \/ i = 4 \/ i = 5) by lia.
+    destruct H as [-> | [-> | [-> | [-> | [-> | ->]]]]];
+    try change (Znth 0 [50; 51; 53; 55; 66; 68] 0) with 50;
+    try change (Znth 1 [50; 51; 53; 55; 66; 68] 0) with 51;
+    try change (Znth 2 [50; 51; 53; 55; 66; 68] 0) with 53;
+    try change (Znth 3 [50; 51; 53; 55; 66; 68] 0) with 55;
+    try change (Znth 4 [50; 51; 53; 55; 66; 68] 0) with 66;
+    try change (Znth 5 [50; 51; 53; 55; 66; 68] 0) with 68;
+    lia.
+  }
+  assert (Hlen : Zlength [50; 51; 53; 55; 66; 68] < 2147483647) by
+    (change (Zlength [50; 51; 53; 55; 66; 68]) with 6; lia).
+  split.
+  - split; [exact Hascii | exact Hnonzero].
+  - split; [exact Hascii | exact Hlen].
+Qed.
+
+Lemma prime_hex_code_range_cases_78 : forall c,
+  0 <= c <= 127 ->
+  prime_hex_code_78 c ->
+  c = 50 \/ c = 51 \/ c = 53 \/ c = 55 \/ c = 66 \/ c = 68.
+Proof.
+  intros c Hrange Hprime.
+  unfold prime_hex_code_78, is_prime_hex_z_78, ascii_of_z_78 in Hprime.
+  assert (Hc : Z.of_nat (Z.to_nat c) = c) by (apply Z2Nat.id; lia).
+  remember (Z.to_nat c) as n eqn:Hn.
+  do 128
+    (destruct n as [| n];
+     cbn in Hprime;
+     try (assert (c = 50 \/ c = 51 \/ c = 53 \/ c = 55 \/ c = 66 \/ c = 68) by lia; tauto);
+     try discriminate).
+Qed.
+
+Lemma prime_hex_code_key_index_78 : forall i c,
+  0 <= i < string_length key_payload_78 ->
+  Znth i key_payload_78 0 = c ->
+  prime_hex_code_78 c.
+Proof.
+  intros i c Hi Hc.
+  unfold key_payload_78, string_length in Hi, Hc.
+  rewrite Zlength_correct in Hi.
+  assert (i = 0 \/ i = 1 \/ i = 2 \/ i = 3 \/ i = 4 \/ i = 5) by (cbn in Hi; lia).
+  destruct H as [-> | [-> | [-> | [-> | [-> | ->]]]]];
+    cbn in Hc; subst c; reflexivity.
+Qed.
+
+Lemma strchr_result_key_hit_prime_78 : forall c ret base,
+  c <> 0 ->
+  strchr_result key_payload_78 c ret base ->
+  ret <> 0 ->
+  prime_hex_code_78 c.
+Proof.
+  intros c ret base Hc0 Hres Hret.
+  unfold strchr_result in Hres.
+  destruct Hres as [Hhit | Hmiss].
+  - destruct Hhit as [i [Hi [Hci [_ [_ _]]]]].
+    eapply prime_hex_code_key_index_78; eauto.
+  - destruct Hmiss as [_ [[Hz _] | [_ Hzero]]].
+    + contradiction.
+    + lia.
+Qed.
+
+Lemma strchr_result_key_miss_not_prime_78 : forall c base,
+  0 <= c <= 127 ->
+  strchr_result key_payload_78 c 0 base ->
+  ~ prime_hex_code_78 c.
+Proof.
+  intros c base Hrange Hres Hprime.
+  unfold strchr_result in Hres.
+  destruct Hres as [[i [_ [_ [_ [_ Hret]]]]] | [Hnone _]].
+  - contradiction.
+  - pose proof (prime_hex_code_range_cases_78 c Hrange Hprime) as Hcases.
+    unfold key_payload_78, string_length in Hnone.
+    destruct Hcases as [-> | [-> | [-> | [-> | [-> | ->]]]]].
+    + specialize (Hnone 0 ltac:(cbn; lia)); vm_compute in Hnone; lia.
+    + specialize (Hnone 1 ltac:(cbn; lia)); vm_compute in Hnone; lia.
+    + specialize (Hnone 2 ltac:(cbn; lia)); vm_compute in Hnone; lia.
+    + specialize (Hnone 3 ltac:(cbn; lia)); vm_compute in Hnone; lia.
+    + specialize (Hnone 4 ltac:(cbn; lia)); vm_compute in Hnone; lia.
+    + specialize (Hnone 5 ltac:(cbn; lia)); vm_compute in Hnone; lia.
+Qed.
+
+Lemma hex_final_from_safe_78 : forall s count,
+  hex_count_safe_78 s ->
+  hex_count_state_78 s (string_length s) count ->
+  hex_final_78 s count.
+Proof.
+  intros s count Hsafe Hstate.
+  unfold hex_count_safe_78 in Hsafe.
+  destruct Hsafe as [_ [_ [_ Hfinal]]].
+  apply Hfinal; assumption.
+Qed.
+
+Lemma hex_hit_from_safe_78 : forall s i count,
+  hex_count_safe_78 s ->
+  hex_count_state_78 s i (count - 1) ->
+  0 <= i < string_length s ->
+  prime_hex_code_78 (Znth i (c_string s) 0) ->
+  hex_hit_step_78 s i count.
+Proof.
+  intros s i count Hsafe Hstate Hi Hprime.
+  unfold hex_count_safe_78 in Hsafe.
+  destruct Hsafe as [_ [Hhit _]].
+  apply Hhit; assumption.
+Qed.
+
+Lemma hex_miss_from_safe_78 : forall s i count,
+  hex_count_safe_78 s ->
+  hex_count_state_78 s i count ->
+  0 <= i < string_length s ->
+  ~ prime_hex_code_78 (Znth i (c_string s) 0) ->
+  hex_miss_step_78 s i count.
+Proof.
+  intros s i count Hsafe Hstate Hi Hmiss.
+  unfold hex_count_safe_78 in Hsafe.
+  destruct Hsafe as [_ [_ [Hmiss_step _]]].
+  apply Hmiss_step; assumption.
+Qed.
